@prefix :      <file:///home/bjorninge/eclipse-workspace/TiltScriptGenerator/#> .
@prefix obda:  <https://w3id.org/obda/vocabulary#> .
@prefix owl:   <http://www.w3.org/2002/07/owl#> .
@prefix rdf:   <http://www.w3.org/1999/02/22-rdf-syntax-ns#> .
@prefix xml:   <http://www.w3.org/XML/1998/namespace> .
@prefix xsd:   <http://www.w3.org/2001/XMLSchema#> .
@prefix rdfs:  <http://www.w3.org/2000/01/rdf-schema#> .

<http://www.uia.no/jpn/tilt#Hyperpnea>
        a                    owl:Class ;
        rdfs:comment         "Hyperpnea (finding)\n\nSCTID: 180928006\n\n180928006 | Hyperpnea (finding) |\n  en   Hyperpnoea\n  en   Hyperpnea\n  en   Hyperpnea (finding)" ;
        rdfs:subClassOf      <http://www.uia.no/jpn/tilt#Respiratory_rate_AND/OR_rhythm_finding> ;
        owl:equivalentClass  [ a               owl:Restriction ;
                               owl:hasValue    "180928006"^^xsd:long ;
                               owl:onProperty  <http://www.uia.no/jpn/tilt#hasSCTID>
                             ] .

<http://www.uia.no/jpn/tilt#On_examination_Diastolic_blood_pressure_reading>
        a                    owl:Class ;
        rdfs:comment         "On examination - Diastolic blood pressure reading (finding)\n\nSCTID: 163031004\n\n163031004 | On examination - Diastolic blood pressure reading (finding) |\n  en   O/E - Diastolic BP reading\n  en   On examination - Diastolic blood pressure reading (finding)\n  en   On examination - Diastolic blood pressure reading\n  en   On examination - Diastolic BP reading" ;
        rdfs:subClassOf      <http://www.uia.no/jpn/tilt#Finding_of_systemic_arterial_pressure> ;
        owl:equivalentClass  [ a               owl:Restriction ;
                               owl:hasValue    "163031004"^^xsd:long ;
                               owl:onProperty  <http://www.uia.no/jpn/tilt#hasSCTID>
                             ] .

<http://www.uia.no/jpn/tilt#CharlieData_18>
        a       <http://www.uia.no/jpn/tilt#SNOWMEDCTSimulatedinput> ;
        <http://www.uia.no/jpn/tilt#hasSCTID>
                "301147003"^^xsd:long ;
        <http://www.uia.no/jpn/tilt#hasTypeName>
                "Pulse_rate_finding" ;
        <http://www.uia.no/jpn/tilt#hasValue>
                <http://www.uia.no/jpn/tilt#CharlieData_18_Value> .

<http://www.uia.no/jpn/tilt#hasHumanName>
        a            owl:DatatypeProperty ;
        rdfs:domain  <http://www.uia.no/jpn/tilt#Human> ;
        rdfs:range   xsd:string .

<http://www.uia.no/jpn/tilt#CharlieData_6>
        a       <http://www.uia.no/jpn/tilt#SNOWMEDCTSimulatedinput> ;
        <http://www.uia.no/jpn/tilt#hasSCTID>
                "1023001"^^xsd:long ;
        <http://www.uia.no/jpn/tilt#hasTypeName>
                "Apnea" ;
        <http://www.uia.no/jpn/tilt#hasValue>
                <http://www.uia.no/jpn/tilt#CharlieData_6_Value> .

<http://www.uia.no/jpn/tilt#Charlie>
        a       <http://www.uia.no/jpn/tilt#Human> ;
        <http://www.uia.no/jpn/tilt#hasHumanAddress>
                "London" ;
        <http://www.uia.no/jpn/tilt#hasHumanName>
                "Charlie" .

<http://www.uia.no/jpn/tilt#Consciousness_related_finding>
        a                    owl:Class ;
        rdfs:comment         "Consciousness related finding (finding)\n\nSCTID: 106167005\n\n106167005 | Consciousness related finding (finding) |\n  en   Consciousness related finding\n  en   Consciousness related finding (finding)\n  en   Consciousness" ;
        rdfs:subClassOf      <http://www.uia.no/jpn/tilt#Consciousness_and/or_awareness_finding> ;
        owl:disjointWith     <http://www.uia.no/jpn/tilt#Finding_of_mental_alertness> ;
        owl:equivalentClass  [ a               owl:Restriction ;
                               owl:hasValue    "106167005"^^xsd:long ;
                               owl:onProperty  <http://www.uia.no/jpn/tilt#hasSCTID>
                             ] .

<http://www.uia.no/jpn/tilt#hasSimulatedInputData>
        a            owl:ObjectProperty ;
        rdfs:domain  <http://www.uia.no/jpn/tilt#SimulatedInputDataSequence> ;
        rdfs:range   <http://www.uia.no/jpn/tilt#SimulatedInputData> .

<http://www.uia.no/jpn/tilt#hasInteraction>
        a            owl:ObjectProperty ;
        rdfs:domain  <http://www.uia.no/jpn/tilt#DrugClass> ;
        rdfs:range   <http://www.uia.no/jpn/tilt#Interaction> .

<http://www.uia.no/jpn/tilt#Drug_Levaxin_ActiveIngredient>
        a       <http://www.uia.no/jpn/tilt#ActiveIngredient> , owl:NamedIndividual ;
        <http://www.uia.no/jpn/tilt#hasAmountInOneDosageForm>
                <http://www.uia.no/jpn/tilt#Drug_Levaxin_Value> ;
        <http://www.uia.no/jpn/tilt#hasDrug>
                <http://www.uia.no/jpn/tilt#Drug_Levaxin_Drug> ;
        <http://www.uia.no/jpn/tilt#hasIngredientName>
                "laktosemonohydrat" .

<http://www.uia.no/jpn/tilt#Responds_to_pain>
        a                    owl:Class ;
        rdfs:comment         "Responds to pain (finding)\n\nSCTID: 450847001\n\n450847001 | Responds to pain (finding) |\n  en   Responds to pain (finding)\n  en   Responds to pain" ;
        rdfs:subClassOf      <http://www.uia.no/jpn/tilt#Finding_of_response_to_pain> ;
        owl:equivalentClass  [ a               owl:Restriction ;
                               owl:hasValue    "450847001"^^xsd:long ;
                               owl:onProperty  <http://www.uia.no/jpn/tilt#hasSCTID>
                             ] .

<http://www.uia.no/jpn/tilt#Finding_related_to_abillity_to_process_information>
        a                    owl:Class ;
        rdfs:comment         "Finding related to ability to process information (finding)\n\nSCTID: 365715000\n\n365715000 | Finding related to ability to process information (finding) |\n  en   Finding related to ability to process information\n  en   Finding related to ability to process information (finding)" ;
        rdfs:subClassOf      <http://www.uia.no/jpn/tilt#Cognitive_function_finding> ;
        owl:equivalentClass  [ a               owl:Restriction ;
                               owl:hasValue    "365715000"^^xsd:long ;
                               owl:onProperty  <http://www.uia.no/jpn/tilt#hasSCTID>
                             ] .

<http://www.uia.no/jpn/tilt#General_characteristic_of_patient>
        a                    owl:Class ;
        rdfs:comment         "General characteristic of patient (observable entity)\n\nSCTID: 363789004\n\n363789004 | General characteristic of patient (observable entity) |\n  en   General characteristic of patient\n  en   General characteristic of patient (observable entity)" ;
        rdfs:subClassOf      <http://www.uia.no/jpn/tilt#Clinical_history_examination_observable> ;
        owl:equivalentClass  [ a               owl:Restriction ;
                               owl:hasValue    "363789004"^^xsd:long ;
                               owl:onProperty  <http://www.uia.no/jpn/tilt#hasSCTID>
                             ] .

<http://www.uia.no/jpn/tilt#CharlieData_26>
        a       <http://www.uia.no/jpn/tilt#SNOWMEDCTSimulatedinput> ;
        <http://www.uia.no/jpn/tilt#hasSCTID>
                "297976006"^^xsd:long ;
        <http://www.uia.no/jpn/tilt#hasTypeName>
                "Finding_of_temperature_of_skin" ;
        <http://www.uia.no/jpn/tilt#hasValue>
                <http://www.uia.no/jpn/tilt#CharlieData_26_Value> .

<http://www.uia.no/jpn/tilt#WarfarinLevotyroksinnatriumInteraction>
        a       <http://www.uia.no/jpn/tilt#Interaction> , owl:NamedIndividual ;
        <http://www.uia.no/jpn/tilt#hasDrugClasses>
                <http://www.uia.no/jpn/tilt#DrugClass_Warfarin> , <http://www.uia.no/jpn/tilt#DrugClass_Analgesics> ;
        <http://www.uia.no/jpn/tilt#hasInteractionDescription>
                "Increased INR with raised probabillity of bleeding" ;
        <http://www.uia.no/jpn/tilt#hasInteractionName>
                "Warfarin and Levotyroksinnatrium interaction" .

<http://www.uia.no/jpn/tilt#General_body_state_finding>
        a                    owl:Class ;
        rdfs:comment         "General body state finding (finding)\n\nSCTID: 82832008\n\n82832008 | General body state finding (finding) |\n  en   General body state finding\n  en   General body state finding (finding)\n  en   General well-being" ;
        rdfs:subClassOf      <http://www.uia.no/jpn/tilt#General_finding_of_observation_of_patient> ;
        owl:equivalentClass  [ a               owl:Restriction ;
                               owl:hasValue    "82832008"^^xsd:long ;
                               owl:onProperty  <http://www.uia.no/jpn/tilt#hasSCTID>
                             ] .

<http://www.uia.no/jpn/tilt#Finding_of_temperature_of_skin>
        a                    owl:Class ;
        rdfs:comment         "Finding of temperature of skin (finding)\n\nSCTID: 297976006\n\n297976006 | Finding of temperature of skin (finding) |\n  en   Finding of temperature of skin\n  en   Finding of temperature of skin (finding)\n  en   Observation of temperature of skin" ;
        rdfs:subClassOf      <http://www.uia.no/jpn/tilt#Body_temperature_finding> ;
        rdfs:subClassOf      [ a                            owl:Restriction ;
                               owl:maxQualifiedCardinality  "1"^^xsd:nonNegativeInteger ;
                               owl:onClass                  <http://www.uia.no/jpn/tilt#Value> ;
                               owl:onProperty               <http://www.uia.no/jpn/tilt#hasValue>
                             ] ;
        owl:equivalentClass  [ a               owl:Restriction ;
                               owl:hasValue    "297976006"^^xsd:long ;
                               owl:onProperty  <http://www.uia.no/jpn/tilt#hasSCTID>
                             ] .

<http://www.uia.no/jpn/tilt#Body_temperature>
        a                    owl:Class ;
        rdfs:comment         "Body temperature (observable entity)\n\nSCTID: 386725007\n\n386725007 | Body temperature (observable entity) |\n  en   Body temperature (observable entity)\n  en   Body temperature\n  en   BT - Body temperature\n  en   Body temperature - observation" ;
        rdfs:subClassOf      <http://www.uia.no/jpn/tilt#General_characteristic_of_patient> ;
        owl:equivalentClass  [ a               owl:Restriction ;
                               owl:hasValue    "386725007"^^xsd:long ;
                               owl:onProperty  <http://www.uia.no/jpn/tilt#hasSCTID>
                             ] .

<http://www.uia.no/jpn/tilt#Clinical_finding>
        a                    owl:Class ;
        rdfs:comment         "Clinical finding (finding)\n\nSCTID: 404684003\n\n404684003 | Clinical finding (finding) |\n  en   Clinical finding (finding)\n  en   Clinical finding" ;
        rdfs:subClassOf      <http://www.uia.no/jpn/tilt#SNOMED_CT_CONCEPT> ;
        owl:equivalentClass  [ a               owl:Restriction ;
                               owl:hasValue    "404684003"^^xsd:long ;
                               owl:onProperty  <http://www.uia.no/jpn/tilt#hasSCTID>
                             ] .

<http://www.uia.no/jpn/tilt#hasEstimatedHumanState>
        a            owl:ObjectProperty ;
        rdfs:domain  <http://www.uia.no/jpn/tilt#Human> ;
        rdfs:range   <http://www.uia.no/jpn/tilt#HumanState> .

<http://www.uia.no/jpn/tilt#Pain>
        a                    owl:Class ;
        rdfs:comment         "Pain (finding)\n\nSCTID: 22253000\n\n22253000 | Pain (finding) |\n  en   Pain\n  en   Dolor\n  en   Painful\n  en   Part hurts\n  en   Pain (finding)\n  en   Pain observations" ;
        rdfs:subClassOf      <http://www.uia.no/jpn/tilt#Pain/sensation_finding> ;
        owl:equivalentClass  [ a               owl:Restriction ;
                               owl:hasValue    "22253000"^^xsd:long ;
                               owl:onProperty  <http://www.uia.no/jpn/tilt#hasSCTID>
                             ] .

<http://www.uia.no/jpn/tilt#hasDefinedDailyDose>
        a           owl:ObjectProperty ;
        rdfs:range  <http://www.uia.no/jpn/tilt#Value> .

<http://www.uia.no/jpn/tilt#Drug_Levaxin_Drug>
        a       <http://www.uia.no/jpn/tilt#Drug> , owl:NamedIndividual ;
        <http://www.uia.no/jpn/tilt#hasArticleNumber>
                "H03A A01" ;
        <http://www.uia.no/jpn/tilt#hasDefinedDailyDose>
                <http://www.uia.no/jpn/tilt#Drug_Levaxin_Value> ;
        <http://www.uia.no/jpn/tilt#hasDosageForm>
                "pills" ;
        <http://www.uia.no/jpn/tilt#hasDrugName>
                "Levaxin" ;
        <http://www.uia.no/jpn/tilt#hasIngredient>
                <http://www.uia.no/jpn/tilt#Drug_Levaxin_ActiveIngredient> ;
        <http://www.uia.no/jpn/tilt#hasNumOfDosageForms>
                "Individuell dosering" .

<http://www.uia.no/jpn/tilt#hasIngredient>
        a            owl:ObjectProperty ;
        rdfs:domain  <http://www.uia.no/jpn/tilt#Drug> ;
        rdfs:range   <http://www.uia.no/jpn/tilt#Ingredient> .

<http://www.uia.no/jpn/tilt#CharlieData_16_Value>
        a       <http://www.uia.no/jpn/tilt#Value> ;
        <http://www.uia.no/jpn/tilt#hasTime>
                "5764" ;
        <http://www.uia.no/jpn/tilt#hasValueType>
                "xsd:float" ;
        <http://www.uia.no/jpn/tilt#hasValueUnit>
                "Unit" ;
        <http://www.uia.no/jpn/tilt#hasValueValue>
                "632.0" .

<http://www.uia.no/jpn/tilt#CharlieData_13>
        a       <http://www.uia.no/jpn/tilt#SNOWMEDCTSimulatedinput> ;
        <http://www.uia.no/jpn/tilt#hasSCTID>
                "301147003"^^xsd:long ;
        <http://www.uia.no/jpn/tilt#hasTypeName>
                "Pulse_rate_finding" ;
        <http://www.uia.no/jpn/tilt#hasValue>
                <http://www.uia.no/jpn/tilt#CharlieData_13_Value> .

<http://www.uia.no/jpn/tilt#Vital_sign_finding>
        a                    owl:Class ;
        rdfs:comment         "Vital signs finding (finding)\n\nSCTID: 118227000\n\n118227000 | Vital signs finding (finding) |\n  en   Vital signs finding\n  en   Vital signs finding (finding)" ;
        rdfs:subClassOf      <http://www.uia.no/jpn/tilt#General_body_state_finding> ;
        owl:equivalentClass  [ a               owl:Restriction ;
                               owl:hasValue    "118227000"^^xsd:long ;
                               owl:onProperty  <http://www.uia.no/jpn/tilt#hasSCTID>
                             ] .

<http://www.uia.no/jpn/tilt#On_examination_Arterial_pressure_index_normal>
        a                    owl:Class ;
        rdfs:comment         "On examination - Arterial pressure index normal (finding)\n\nSCTID: 310356000\n\n310356000 | On examination - Arterial pressure index normal (finding) |\n  en   O/E - Arterial pressure index normal\n  en   On examination - Arterial pressure index normal (finding)\n  en   On examination - Arterial pressure index normal" ;
        rdfs:subClassOf      <http://www.uia.no/jpn/tilt#Finding_of_systemic_arterial_pressure> ;
        owl:equivalentClass  [ a               owl:Restriction ;
                               owl:hasValue    "310356000"^^xsd:long ;
                               owl:onProperty  <http://www.uia.no/jpn/tilt#hasSCTID>
                             ] .

<http://www.uia.no/jpn/tilt#CharlieData_1>
        a       <http://www.uia.no/jpn/tilt#SNOWMEDCTSimulatedinput> ;
        <http://www.uia.no/jpn/tilt#hasSCTID>
                "163030003"^^xsd:long ;
        <http://www.uia.no/jpn/tilt#hasTypeName>
                "On_examination_Systolic_blood_pressure_reading" ;
        <http://www.uia.no/jpn/tilt#hasValue>
                <http://www.uia.no/jpn/tilt#CharlieData_1_Value> .

<http://www.uia.no/jpn/tilt#hasAmountInOneDosageForm>
        a            owl:ObjectProperty ;
        rdfs:domain  <http://www.uia.no/jpn/tilt#Ingredient> ;
        rdfs:range   <http://www.uia.no/jpn/tilt#Value> .

<http://www.uia.no/jpn/tilt#Clinical_history_and_observation_finding>
        a                    owl:Class ;
        rdfs:comment         "Clinical history and observation findings (finding)\n\nSCTID: 250171008\n\n250171008 | Clinical history and observation findings (finding) |\n  en   Clinical history and observation findings\n  en   Clinical history and observation findings (finding)\n  en   Clinical history and observations" ;
        rdfs:subClassOf      <http://www.uia.no/jpn/tilt#Clinical_finding> ;
        owl:equivalentClass  [ a               owl:Restriction ;
                               owl:hasValue    "250171008"^^xsd:long ;
                               owl:onProperty  <http://www.uia.no/jpn/tilt#hasSCTID>
                             ] .

<http://www.uia.no/jpn/tilt#Value>
        a                owl:Class , owl:DatatypeProperty ;
        rdfs:comment     "We have already placed all the data properties to functional, so, in theory, we do not need to set the max to 1, it is implicit in the function functional. But for brevity, we add an extra layer of understanding." ;
        rdfs:subClassOf  [ a            owl:Class ;
                           owl:unionOf  ( [ a                         owl:Restriction ;
                                            owl:onDataRange           xsd:string ;
                                            owl:onProperty            <http://www.uia.no/jpn/tilt#hasValueValue> ;
                                            owl:qualifiedCardinality  "1"^^xsd:nonNegativeInteger
                                          ]
                                          [ a                            owl:Restriction ;
                                            owl:maxQualifiedCardinality  "1"^^xsd:nonNegativeInteger ;
                                            owl:onDataRange              xsd:long ;
                                            owl:onProperty               <http://www.uia.no/jpn/tilt#hasTime>
                                          ]
                                          [ a                            owl:Restriction ;
                                            owl:maxQualifiedCardinality  "1"^^xsd:nonNegativeInteger ;
                                            owl:onDataRange              xsd:string ;
                                            owl:onProperty               <http://www.uia.no/jpn/tilt#hasValueType>
                                          ]
                                          [ a                            owl:Restriction ;
                                            owl:maxQualifiedCardinality  "1"^^xsd:nonNegativeInteger ;
                                            owl:onDataRange              xsd:string ;
                                            owl:onProperty               <http://www.uia.no/jpn/tilt#hasValueUnit>
                                          ]
                                        )
                         ] .

<http://www.uia.no/jpn/tilt#Pain/sensation_finding>
        a                    owl:Class ;
        rdfs:comment         "Pain / sensation finding (finding)\n\nSCTID: 276435006\n\n276435006 | Pain / sensation finding (finding) |\n  en   Pain / sensation finding\n  en   Pain / sensation finding (finding)\n  en   Pain and sensation" ;
        rdfs:subClassOf      <http://www.uia.no/jpn/tilt#Sensory_nervous_system_finding> ;
        owl:equivalentClass  [ a               owl:Restriction ;
                               owl:hasValue    "276435006"^^xsd:long ;
                               owl:onProperty  <http://www.uia.no/jpn/tilt#hasSCTID>
                             ] .

<http://www.uia.no/jpn/tilt#CharlieData_7_Value>
        a       <http://www.uia.no/jpn/tilt#Value> ;
        <http://www.uia.no/jpn/tilt#hasTime>
                "1236" ;
        <http://www.uia.no/jpn/tilt#hasValueType>
                "xsd:float" ;
        <http://www.uia.no/jpn/tilt#hasValueUnit>
                "Unit" ;
        <http://www.uia.no/jpn/tilt#hasValueValue>
                "376.0" .

<http://www.uia.no/jpn/tilt#Respiratory_rate>
        a                    owl:Class ;
        rdfs:comment         "Respiratory rate (observable entity)\n\nSCTID: 86290005\n\n86290005 | Respiratory rate (observable entity) |\n  en   Respiratory rate\n  en   Respiratory rate (observable entity)\n  en   BR - Breathing rate\n  en   Respiratory frequency\n  en   Breathing rate\n  en   RR - Respiratory rate\n  en   Rate of respiration" ;
        rdfs:subClassOf      <http://www.uia.no/jpn/tilt#Respiratory_measure> ;
        owl:equivalentClass  [ a               owl:Restriction ;
                               owl:hasValue    "86290005"^^xsd:long ;
                               owl:onProperty  <http://www.uia.no/jpn/tilt#hasSCTID>
                             ] .

<http://www.uia.no/jpn/tilt#hasDrugClassName>
        a                   owl:FunctionalProperty , owl:DatatypeProperty ;
        rdfs:domain         <http://www.uia.no/jpn/tilt#DrugClass> ;
        rdfs:range          xsd:string ;
        rdfs:subPropertyOf  owl:topDataProperty .

<http://www.uia.no/jpn/tilt#Human>
        a                owl:Class ;
        rdfs:subClassOf  [ a                         owl:Restriction ;
                           owl:onClass               <http://www.uia.no/jpn/tilt#HumanState> ;
                           owl:onProperty            <http://www.uia.no/jpn/tilt#hasEstimatedHumanState> ;
                           owl:qualifiedCardinality  "1"^^xsd:nonNegativeInteger
                         ] ;
        rdfs:subClassOf  [ a                            owl:Restriction ;
                           owl:minQualifiedCardinality  "0"^^xsd:nonNegativeInteger ;
                           owl:onClass                  <http://www.uia.no/jpn/tilt#Observable_entity> ;
                           owl:onProperty               <http://www.uia.no/jpn/tilt#hasObservableEntity>
                         ] .

<http://www.uia.no/jpn/tilt#hasHumanAddress>
        a            owl:DatatypeProperty ;
        rdfs:domain  <http://www.uia.no/jpn/tilt#Human> ;
        rdfs:range   xsd:string .

<http://www.uia.no/jpn/tilt#CharlieData_21>
        a       <http://www.uia.no/jpn/tilt#SNOWMEDCTSimulatedinput> ;
        <http://www.uia.no/jpn/tilt#hasSCTID>
                "163031004"^^xsd:long ;
        <http://www.uia.no/jpn/tilt#hasTypeName>
                "On_examination_Diastolic_blood_pressure_reading" ;
        <http://www.uia.no/jpn/tilt#hasValue>
                <http://www.uia.no/jpn/tilt#CharlieData_21_Value> .

<http://www.uia.no/jpn/tilt#CharlieData_12_Value>
        a       <http://www.uia.no/jpn/tilt#Value> ;
        <http://www.uia.no/jpn/tilt#hasTime>
                "7367" ;
        <http://www.uia.no/jpn/tilt#hasValueType>
                "xsd:float" ;
        <http://www.uia.no/jpn/tilt#hasValueUnit>
                "Unit" ;
        <http://www.uia.no/jpn/tilt#hasValueValue>
                "26.0" .

<http://www.uia.no/jpn/tilt#CharlieData_9>
        a       <http://www.uia.no/jpn/tilt#SNOWMEDCTSimulatedinput> ;
        <http://www.uia.no/jpn/tilt#hasSCTID>
                "5467003"^^xsd:long ;
        <http://www.uia.no/jpn/tilt#hasTypeName>
                "Normal_respiratory_rhythm" ;
        <http://www.uia.no/jpn/tilt#hasValue>
                <http://www.uia.no/jpn/tilt#CharlieData_9_Value> .

<http://www.uia.no/jpn/tilt#Function>
        a                    owl:Class ;
        rdfs:comment         "Function (observable entity)\n\nSCTID: 246464006\n\n246464006 | Function (observable entity) |\n  en   Function (observable entity)\n  en   Function\n  en   Any function or property that is not mainly morphologic or structural, including both measurable and observable features and physiologic actions" ;
        rdfs:subClassOf      <http://www.uia.no/jpn/tilt#Observable_entity> ;
        owl:equivalentClass  [ a               owl:Restriction ;
                               owl:hasValue    "246464006"^^xsd:long ;
                               owl:onProperty  <http://www.uia.no/jpn/tilt#hasSCTID>
                             ] .

<http://www.uia.no/jpn/tilt#CharlieData_3_Value>
        a       <http://www.uia.no/jpn/tilt#Value> ;
        <http://www.uia.no/jpn/tilt#hasTime>
                "73" ;
        <http://www.uia.no/jpn/tilt#hasValueType>
                "xsd:float" ;
        <http://www.uia.no/jpn/tilt#hasValueUnit>
                "Unit" ;
        <http://www.uia.no/jpn/tilt#hasValueValue>
                "33.8" .

<http://www.uia.no/jpn/tilt#CharlieData_25_Value>
        a       <http://www.uia.no/jpn/tilt#Value> ;
        <http://www.uia.no/jpn/tilt#hasTime>
                "74" ;
        <http://www.uia.no/jpn/tilt#hasValueType>
                "xsd:float" ;
        <http://www.uia.no/jpn/tilt#hasValueUnit>
                "Unit" ;
        <http://www.uia.no/jpn/tilt#hasValueValue>
                "47.0" .

<http://www.uia.no/jpn/tilt#Drug_Euthyrox_Drug>
        a       <http://www.uia.no/jpn/tilt#Drug> , owl:NamedIndividual ;
        <http://www.uia.no/jpn/tilt#hasArticleNumber>
                "H03A A01" ;
        <http://www.uia.no/jpn/tilt#hasDosageForm>
                "pills" ;
        <http://www.uia.no/jpn/tilt#hasDrugName>
                "Euthyrox" ;
        <http://www.uia.no/jpn/tilt#hasIngredient>
                <http://www.uia.no/jpn/tilt#Drug_Euthyrox_ActiveIngredient_Levotyroksinnatrium> ;
        <http://www.uia.no/jpn/tilt#hasNumOfDosageForms>
                "individuell dosering. Pasienten trenger vanligvis bare 1 eller 2 tabletter daglig." .

<http://www.uia.no/jpn/tilt#CodedSimulatedInputData>
        a                owl:Class ;
        rdfs:subClassOf  <http://www.uia.no/jpn/tilt#SimulatedInputData> .

<http://www.uia.no/jpn/tilt#Cardiovascular_function>
        a                    owl:Class ;
        rdfs:comment         "Cardiovascular function (observable entity)\n\nSCTID: 70337006\n\n70337006 | Cardiovascular function (observable entity) |\n  en   Cardiovascular function\n  en   Cardiovascular function (observable entity)" ;
        rdfs:subClassOf      <http://www.uia.no/jpn/tilt#Function> ;
        owl:equivalentClass  [ a               owl:Restriction ;
                               owl:hasValue    "70337006"^^xsd:long ;
                               owl:onProperty  <http://www.uia.no/jpn/tilt#hasSCTID>
                             ] .

<http://www.uia.no/jpn/tilt#CharlieData_21_Value>
        a       <http://www.uia.no/jpn/tilt#Value> ;
        <http://www.uia.no/jpn/tilt#hasTime>
                "1962" ;
        <http://www.uia.no/jpn/tilt#hasValueType>
                "xsd:float" ;
        <http://www.uia.no/jpn/tilt#hasValueUnit>
                "Unit" ;
        <http://www.uia.no/jpn/tilt#hasValueValue>
                "440.0" .

<http://www.uia.no/jpn/tilt#Respiration_observable>
        a                    owl:Class ;
        rdfs:comment         "Respiration observable (observable entity)\n\nSCTID: 364062005\n\n364062005 | Respiration observable (observable entity) |\n  en   Respiration observable\n  en   Respiration observable (observable entity)" ;
        rdfs:subClassOf      <http://www.uia.no/jpn/tilt#Respiratory_observable> ;
        owl:equivalentClass  [ a               owl:Restriction ;
                               owl:hasValue    "364062005"^^xsd:long ;
                               owl:onProperty  <http://www.uia.no/jpn/tilt#hasSCTID>
                             ] .

<http://www.uia.no/jpn/tilt#Psychological_finding>
        a                    owl:Class ;
        rdfs:comment         "Psychological finding (finding)\n\nSCTID: 116367006\n\n116367006 | Psychological finding (finding) |\n  en   Psychological finding\n  en   Psychological finding (finding)" ;
        rdfs:subClassOf      <http://www.uia.no/jpn/tilt#Clinical_history_and_observation_finding> ;
        owl:equivalentClass  [ a               owl:Restriction ;
                               owl:hasValue    "116367006"^^xsd:long ;
                               owl:onProperty  <http://www.uia.no/jpn/tilt#hasSCTID>
                             ] .

<http://www.uia.no/jpn/tilt#Diastolic_blood_pressure>
        a                    owl:Class ;
        rdfs:comment         "Diastolic blood pressure (observable entity)\n\nSCTID: 271650006\n\n271650006 | Diastolic blood pressure (observable entity) |\n  en   Diastolic blood pressure\n  en   Diastolic blood pressure (observable entity)\n  en   DAP - Diastolic arterial pressure\n  en   DBP - Diastolic blood pressure\n  en   Diastolic arterial pressure" ;
        rdfs:subClassOf      <http://www.uia.no/jpn/tilt#Vascular_measure> , <http://www.uia.no/jpn/tilt#Blood_pressure> ;
        owl:equivalentClass  [ a               owl:Restriction ;
                               owl:hasValue    "271650006"^^xsd:long ;
                               owl:onProperty  <http://www.uia.no/jpn/tilt#hasSCTID>
                             ] .

<http://www.uia.no/jpn/tilt#hasDrug>
        a            owl:ObjectProperty ;
        rdfs:domain  <http://www.uia.no/jpn/tilt#Ingredient> ;
        rdfs:range   <http://www.uia.no/jpn/tilt#Drug> .

<http://www.uia.no/jpn/tilt#CharlieData_16>
        a       <http://www.uia.no/jpn/tilt#SNOWMEDCTSimulatedinput> ;
        <http://www.uia.no/jpn/tilt#hasSCTID>
                "310356000"^^xsd:long ;
        <http://www.uia.no/jpn/tilt#hasTypeName>
                "On_examination_Arterial_pressure_index_normal" ;
        <http://www.uia.no/jpn/tilt#hasValue>
                <http://www.uia.no/jpn/tilt#CharlieData_16_Value> .

<http://www.uia.no/jpn/tilt#CharlieData_4>
        a       <http://www.uia.no/jpn/tilt#SNOWMEDCTSimulatedinput> ;
        <http://www.uia.no/jpn/tilt#hasSCTID>
                "297976006"^^xsd:long ;
        <http://www.uia.no/jpn/tilt#hasTypeName>
                "Finding_of_temperature_of_skin" ;
        <http://www.uia.no/jpn/tilt#hasValue>
                <http://www.uia.no/jpn/tilt#CharlieData_4_Value> .

<http://www.uia.no/jpn/tilt#Sim_1>
        a       owl:NamedIndividual , <http://www.uia.no/jpn/tilt#SimulatedInputDataSequence> ;
        <http://www.uia.no/jpn/tilt#hasSimulatedInputData>
                <http://www.uia.no/jpn/tilt#CharlieData_5> , <http://www.uia.no/jpn/tilt#CharlieData_11> , <http://www.uia.no/jpn/tilt#CharlieData_15> , <http://www.uia.no/jpn/tilt#CharlieData_22> , <http://www.uia.no/jpn/tilt#CharlieData_25> , <http://www.uia.no/jpn/tilt#CharlieData_24> , <http://www.uia.no/jpn/tilt#CharlieData_14> , <http://www.uia.no/jpn/tilt#CharlieData_17> , <http://www.uia.no/jpn/tilt#CharlieData_2> , <http://www.uia.no/jpn/tilt#CharlieData_21> , <http://www.uia.no/jpn/tilt#CharlieData_13> , <http://www.uia.no/jpn/tilt#CharlieData_16> , <http://www.uia.no/jpn/tilt#CharlieData_8> , <http://www.uia.no/jpn/tilt#CharlieData_1> , <http://www.uia.no/jpn/tilt#CharlieData_23> , <http://www.uia.no/jpn/tilt#CharlieData_7> , <http://www.uia.no/jpn/tilt#CharlieData_9> , <http://www.uia.no/jpn/tilt#CharlieData_26> , <http://www.uia.no/jpn/tilt#CharlieData_20> , <http://www.uia.no/jpn/tilt#CharlieData_19> , <http://www.uia.no/jpn/tilt#CharlieData_10> , <http://www.uia.no/jpn/tilt#CharlieData_4> , <http://www.uia.no/jpn/tilt#CharlieData_18> , <http://www.uia.no/jpn/tilt#CharlieData_12> , <http://www.uia.no/jpn/tilt#CharlieData_3> , <http://www.uia.no/jpn/tilt#CharlieData_6> .

<http://www.uia.no/jpn/tilt#Respiratory_rate_AND/OR_rhythm_finding>
        a                    owl:Class ;
        rdfs:comment         "Respiratory rate AND/OR rhythm finding (finding)\n\nSCTID: 106049001\n\n106049001 | Respiratory rate AND/OR rhythm finding (finding) |\n  en   Respiratory rate AND/OR rhythm finding\n  en   Respiratory rate AND/OR rhythm finding (finding)" ;
        rdfs:subClassOf      <http://www.uia.no/jpn/tilt#Vital_sign_finding> ;
        owl:equivalentClass  [ a               owl:Restriction ;
                               owl:hasValue    "106049001"^^xsd:long ;
                               owl:onProperty  <http://www.uia.no/jpn/tilt#hasSCTID>
                             ] .

<http://www.uia.no/jpn/tilt#DrugClass_Warfarin>
        a       <http://www.uia.no/jpn/tilt#DrugClass> , owl:NamedIndividual ;
        <http://www.uia.no/jpn/tilt#hasActiveIngredient>
                <http://www.uia.no/jpn/tilt#Drug_Marevan_ActiveIngredient_Warfarinnatrium> ;
        <http://www.uia.no/jpn/tilt#hasDrugClassName>
                "Warfarin" ;
        <http://www.uia.no/jpn/tilt#hasInteraction>
                <http://www.uia.no/jpn/tilt#WarfarinLevotyroksinnatriumInteraction> .

<http://www.uia.no/jpn/tilt#Pulse_function>
        a                    owl:Class ;
        rdfs:comment         "Pulse, function (observable entity)\n\nSCTID: 8499008\n\n8499008 | Pulse, function (observable entity) |\n  en   Pulse\n  en   Pulse, function (observable entity)\n  en   Pulse, function" ;
        rdfs:subClassOf      <http://www.uia.no/jpn/tilt#Cardiovascular_function> ;
        owl:equivalentClass  [ a               owl:Restriction ;
                               owl:hasValue    "8499008"^^xsd:long ;
                               owl:onProperty  <http://www.uia.no/jpn/tilt#hasSCTID>
                             ] .

<http://www.uia.no/jpn/tilt#Finding_of_rate_of_respiration_finding>
        a                    owl:Class ;
        rdfs:comment         "Finding of rate of respiration (finding)\n\nSCTID: 301283003\n\n301283003 | Finding of rate of respiration (finding) |\n  en   Finding of rate of respiration\n  en   Finding of rate of respiration (finding)\n  en   Observation of rate of respiration" ;
        rdfs:subClassOf      <http://www.uia.no/jpn/tilt#Respiratory_rate_AND/OR_rhythm_finding> ;
        rdfs:subClassOf      [ a                            owl:Restriction ;
                               owl:maxQualifiedCardinality  "1"^^xsd:nonNegativeInteger ;
                               owl:onClass                  <http://www.uia.no/jpn/tilt#Value> ;
                               owl:onProperty               <http://www.uia.no/jpn/tilt#hasValue>
                             ] ;
        owl:equivalentClass  [ a               owl:Restriction ;
                               owl:hasValue    "301283003"^^xsd:long ;
                               owl:onProperty  <http://www.uia.no/jpn/tilt#hasSCTID>
                             ] .

<http://www.uia.no/jpn/tilt#Drug_Marevan_Drug>
        a       <http://www.uia.no/jpn/tilt#Drug> , owl:NamedIndividual ;
        <http://www.uia.no/jpn/tilt#hasArticleNumber>
                "B01A A03" ;
        <http://www.uia.no/jpn/tilt#hasDosageForm>
                "pills" ;
        <http://www.uia.no/jpn/tilt#hasDrugName>
                "Marevan" ;
        <http://www.uia.no/jpn/tilt#hasIngredient>
                <http://www.uia.no/jpn/tilt#Drug_Marevan_InactiveIngredient_Lactose> , <http://www.uia.no/jpn/tilt#Drug_Marevan_ActiveIngredient_Warfarinnatrium> ;
        <http://www.uia.no/jpn/tilt#hasNumOfDosageForms>
                "Vanlig dose 1. og 2. dag er 3 tabletter (7,5 mg)." .

<http://www.uia.no/jpn/tilt#CharlieData_24>
        a       <http://www.uia.no/jpn/tilt#SNOWMEDCTSimulatedinput> ;
        <http://www.uia.no/jpn/tilt#hasSCTID>
                "5467003"^^xsd:long ;
        <http://www.uia.no/jpn/tilt#hasTypeName>
                "Normal_respiratory_rhythm" ;
        <http://www.uia.no/jpn/tilt#hasValue>
                <http://www.uia.no/jpn/tilt#CharlieData_24_Value> .

<http://www.uia.no/jpn/tilt#On_examination_Arterial_pressure_index_abnormal>
        a                    owl:Class ;
        rdfs:comment         "On examination - Arterial pressure index abnormal (finding)\n\nSCTID: 310357009\n\n310357009 | On examination - Arterial pressure index abnormal (finding) |\n  en   O/E - Arterial pressure index abnormal\n  en   On examination - Arterial pressure index abnormal (finding)\n  en   On examination - Arterial pressure index abnormal" ;
        rdfs:subClassOf      <http://www.uia.no/jpn/tilt#Finding_of_systemic_arterial_pressure> ;
        owl:equivalentClass  [ a               owl:Restriction ;
                               owl:hasValue    "310357009"^^xsd:long ;
                               owl:onProperty  <http://www.uia.no/jpn/tilt#hasSCTID>
                             ] .

<http://www.uia.no/jpn/tilt#hasInteractionName>
        a                   owl:FunctionalProperty , owl:DatatypeProperty ;
        rdfs:domain         <http://www.uia.no/jpn/tilt#Interaction> ;
        rdfs:range          xsd:string ;
        rdfs:subPropertyOf  owl:topDataProperty .

<http://www.uia.no/jpn/tilt#hasArticleNumber>
        a                   owl:FunctionalProperty , owl:DatatypeProperty ;
        rdfs:domain         [ a            owl:Class ;
                              owl:unionOf  ( <http://www.uia.no/jpn/tilt#Drug> <http://www.uia.no/jpn/tilt#DrugSimulatedInputData> )
                            ] ;
        rdfs:range          xsd:string ;
        rdfs:subPropertyOf  owl:topDataProperty .

<http://www.uia.no/jpn/tilt#Normal_respiratory_rhythm>
        a                    owl:Class ;
        rdfs:comment         "Normal respiratory rhythm (finding)\n\nSCTID: 5467003\n\n5467003 | Normal respiratory rhythm (finding) |\n  en   Normal respiratory rhythm\n  en   Normal respiratory rhythm (finding)" ;
        rdfs:subClassOf      <http://www.uia.no/jpn/tilt#Respiratory_rate_AND/OR_rhythm_finding> ;
        owl:equivalentClass  [ a               owl:Restriction ;
                               owl:hasValue    "5467003"^^xsd:long ;
                               owl:onProperty  <http://www.uia.no/jpn/tilt#hasSCTID>
                             ] .

<http://www.uia.no/jpn/tilt#CharlieData_19_Value>
        a       <http://www.uia.no/jpn/tilt#Value> ;
        <http://www.uia.no/jpn/tilt#hasTime>
                "295" ;
        <http://www.uia.no/jpn/tilt#hasValueType>
                "xsd:float" ;
        <http://www.uia.no/jpn/tilt#hasValueUnit>
                "Unit" ;
        <http://www.uia.no/jpn/tilt#hasValueValue>
                "50.3" .

<http://www.uia.no/jpn/tilt#Observable_entity>
        a                    owl:Class ;
        rdfs:comment         "Observable entity (observable entity)\n\nSCTID: 363787002\n\n363787002 | Observable entity (observable entity) |\n  en   Observable entity\n  en   Observable entity (observable entity)" ;
        rdfs:subClassOf      <http://www.uia.no/jpn/tilt#SNOMED_CT_CONCEPT> ;
        owl:equivalentClass  [ a               owl:Restriction ;
                               owl:hasValue    "363787002"^^xsd:long ;
                               owl:onProperty  <http://www.uia.no/jpn/tilt#hasSCTID>
                             ] .

<http://www.uia.no/jpn/tilt#Cognitive_function_finding>
        a                    owl:Class ;
        rdfs:comment         "Cognitive function finding (finding)\n\nSCTID: 373930000\n\n373930000 | Cognitive function finding (finding) |\n  en   Cognitive function finding (finding)\n  en   Cognitive function finding\n  en   Cognitive function observations" ;
        rdfs:subClassOf      <http://www.uia.no/jpn/tilt#Mental_state,_behavior_and/or_psychosocial_function_finding> ;
        owl:disjointWith     <http://www.uia.no/jpn/tilt#Mentalstate_state_finding> ;
        owl:equivalentClass  [ a               owl:Restriction ;
                               owl:hasValue    "373930000"^^xsd:long ;
                               owl:onProperty  <http://www.uia.no/jpn/tilt#hasSCTID>
                             ] .

<http://www.uia.no/jpn/tilt#Able_to_process_information>
        a                    owl:Class ;
        rdfs:comment         "Able to process information (finding)\n\nSCTID: 307083000\n\n307083000 | Able to process information (finding) |\n  en   Able to process information\n  en   Able to process information (finding)" ;
        rdfs:subClassOf      <http://www.uia.no/jpn/tilt#Finding_related_to_abillity_to_process_information> ;
        owl:equivalentClass  [ a               owl:Restriction ;
                               owl:hasValue    "307083000"^^xsd:long ;
                               owl:onProperty  <http://www.uia.no/jpn/tilt#hasSCTID>
                             ] .

<http://www.uia.no/jpn/tilt#CharlieData_11>
        a       <http://www.uia.no/jpn/tilt#SNOWMEDCTSimulatedinput> ;
        <http://www.uia.no/jpn/tilt#hasSCTID>
                "310357009"^^xsd:long ;
        <http://www.uia.no/jpn/tilt#hasTypeName>
                "On_examination_Arterial_pressure_index_abnormal" ;
        <http://www.uia.no/jpn/tilt#hasValue>
                <http://www.uia.no/jpn/tilt#CharlieData_11_Value> .

<http://www.uia.no/jpn/tilt#InactiveIngredient>
        a                owl:Class ;
        rdfs:comment     "This class is supressed, no variables given. Class is then primitive" ;
        rdfs:subClassOf  <http://www.uia.no/jpn/tilt#Ingredient> .

<http://www.uia.no/jpn/tilt#Mentalstate_state_finding>
        a                    owl:Class ;
        rdfs:comment         "Mental state finding (finding)\n\nSCTID: 36456004\n\n36456004 | Mental state finding (finding) |\n  en   Mental state\n  en   Mental status\n  en   Mental state finding\n  en   Mental state finding (finding)" ;
        rdfs:subClassOf      <http://www.uia.no/jpn/tilt#Mental_state,_behavior_and/or_psychosocial_function_finding> ;
        owl:equivalentClass  [ a               owl:Restriction ;
                               owl:hasValue    "36456004"^^xsd:long ;
                               owl:onProperty  <http://www.uia.no/jpn/tilt#hasSCTID>
                             ] .

<http://www.uia.no/jpn/tilt#CharlieData_19>
        a       <http://www.uia.no/jpn/tilt#SNOWMEDCTSimulatedinput> ;
        <http://www.uia.no/jpn/tilt#hasSCTID>
                "180928006"^^xsd:long ;
        <http://www.uia.no/jpn/tilt#hasTypeName>
                "Hyperpnea" ;
        <http://www.uia.no/jpn/tilt#hasValue>
                <http://www.uia.no/jpn/tilt#CharlieData_19_Value> .

<http://www.uia.no/jpn/tilt#CharlieData_15_Value>
        a       <http://www.uia.no/jpn/tilt#Value> ;
        <http://www.uia.no/jpn/tilt#hasTime>
                "653" ;
        <http://www.uia.no/jpn/tilt#hasValueType>
                "xsd:float" ;
        <http://www.uia.no/jpn/tilt#hasValueUnit>
                "Unit" ;
        <http://www.uia.no/jpn/tilt#hasValueValue>
                "62.0" .

<http://www.uia.no/jpn/tilt#CharlieData_7>
        a       <http://www.uia.no/jpn/tilt#SNOWMEDCTSimulatedinput> ;
        <http://www.uia.no/jpn/tilt#hasSCTID>
                "5467003"^^xsd:long ;
        <http://www.uia.no/jpn/tilt#hasTypeName>
                "Normal_respiratory_rhythm" ;
        <http://www.uia.no/jpn/tilt#hasValue>
                <http://www.uia.no/jpn/tilt#CharlieData_7_Value> .

<http://www.uia.no/jpn/tilt#CharlieData_6_Value>
        a       <http://www.uia.no/jpn/tilt#Value> ;
        <http://www.uia.no/jpn/tilt#hasTime>
                "4" ;
        <http://www.uia.no/jpn/tilt#hasValueType>
                "xsd:float" ;
        <http://www.uia.no/jpn/tilt#hasValueUnit>
                "Unit" ;
        <http://www.uia.no/jpn/tilt#hasValueValue>
                "36.0" .

<http://www.uia.no/jpn/tilt#On_examination_Systolic_blood_pressure_reading>
        a                    owl:Class ;
        rdfs:comment         "On examination - Systolic blood pressure reading (finding)\n\nSCTID: 163030003\n\n163030003 | On examination - Systolic blood pressure reading (finding) |\n  en   O/E - Systolic BP reading\n  en   On examination - Systolic BP reading\n  en   On examination - Systolic blood pressure reading (finding)\n  en   On examination - Systolic blood pressure reading" ;
        rdfs:subClassOf      <http://www.uia.no/jpn/tilt#Finding_of_systemic_arterial_pressure> ;
        rdfs:subClassOf      [ a                            owl:Restriction ;
                               owl:maxQualifiedCardinality  "1"^^xsd:nonNegativeInteger ;
                               owl:onClass                  <http://www.uia.no/jpn/tilt#Value> ;
                               owl:onProperty               <http://www.uia.no/jpn/tilt#hasValue>
                             ] ;
        owl:equivalentClass  [ a               owl:Restriction ;
                               owl:hasValue    "163030003"^^xsd:long ;
                               owl:onProperty  <http://www.uia.no/jpn/tilt#hasSCTID>
                             ] .

<http://www.uia.no/jpn/tilt#Respiratory_observable>
        a                    owl:Class ;
        rdfs:comment         "Respiratory observable (observable entity)\n\nSCTID: 364048003\n\n364048003 | Respiratory observable (observable entity) |\n  en   Respiratory observable\n  en   Respiratory observable (observable entity)" ;
        rdfs:subClassOf      <http://www.uia.no/jpn/tilt#Clinical_history_examination_observable> ;
        owl:equivalentClass  [ a               owl:Restriction ;
                               owl:hasValue    "364048003"^^xsd:long ;
                               owl:onProperty  <http://www.uia.no/jpn/tilt#hasSCTID>
                             ] .

<http://www.uia.no/jpn/tilt#hasInteractionDescription>
        a                   owl:FunctionalProperty , owl:DatatypeProperty ;
        rdfs:domain         <http://www.uia.no/jpn/tilt#Interaction> ;
        rdfs:range          xsd:string ;
        rdfs:subPropertyOf  owl:topDataProperty .

<http://www.uia.no/jpn/tilt#hasStrengthOfDosageForm>
        a           owl:ObjectProperty ;
        rdfs:range  <http://www.uia.no/jpn/tilt#Value> .

<http://www.uia.no/jpn/tilt#DrugClass_Analgesics>
        a       <http://www.uia.no/jpn/tilt#DrugClass> , owl:NamedIndividual ;
        <http://www.uia.no/jpn/tilt#hasActiveIngredient>
                <http://www.uia.no/jpn/tilt#Drug_Euthyrox_ActiveIngredient_Levotyroksinnatrium> ;
        <http://www.uia.no/jpn/tilt#hasDrugClassName>
                "Analgesics" ;
        <http://www.uia.no/jpn/tilt#hasInteraction>
                <http://www.uia.no/jpn/tilt#WarfarinLevotyroksinnatriumInteraction> .

<http://www.uia.no/jpn/tilt#Finding_of_systemic_arterial_pressure>
        a                    owl:Class ;
        rdfs:comment         "Finding of systemic arterial pressure (finding)\n\nSCTID: 301140001\n\n301140001 | Finding of systemic arterial pressure (finding) |\n  en   Finding of systemic arterial pressure\n  en   Finding of systemic arterial pressure (finding)\n  en   Observation of systemic arterial pressure" ;
        rdfs:subClassOf      <http://www.uia.no/jpn/tilt#Blood_pressure_finding> ;
        owl:equivalentClass  [ a               owl:Restriction ;
                               owl:hasValue    "301140001"^^xsd:long ;
                               owl:onProperty  <http://www.uia.no/jpn/tilt#hasSCTID>
                             ] .

<http://www.uia.no/jpn/tilt#SNOMED_CT_CONCEPT>
        a                    owl:Class ;
        rdfs:comment         "SNOMED CT Concept (SNOMED RT+CTV3)\n\nSCTID: 138875005\n\n138875005 | SNOMED CT Concept (SNOMED RT+CTV3) |\n  en   SNOMED CT Concept\n  en   SNOMED CT Concept (SNOMED RT+CTV3)\n  en   SNOMED CT has been created by combining SNOMED RT and a computer-based nomenclature and classification known as Read Codes Version 3, which was created on behalf of the U.K. Department of Health.\n  en   © 2002-2018 International Health Terminology Standards Development Organisation (IHTSDO). All rights reserved. SNOMED CT®, was originally created by The College of American Pathologists. \"SNOMED\" and \"SNOMED CT\" are registered trademarks of the IHTSDO.\n  en   SNOMED Clinical Terms version: 20180731 [R] (July 2018 Release)" ;
        rdfs:seeAlso         "http://browser.ihtsdotools.org/?perspective=full&conceptId1=138875005&edition=en-edition&release=v20180731&server=http://browser.ihtsdotools.org/api/v1/snomed&langRefset=900000000000509007" ;
        owl:equivalentClass  [ a               owl:Restriction ;
                               owl:hasValue    "138875005"^^xsd:long ;
                               owl:onProperty  <http://www.uia.no/jpn/tilt#hasSCTID>
                             ] ;
        owl:versionInfo      "July 2018 Release" .

<http://www.uia.no/jpn/tilt#HumanState>
        a                owl:Class ;
        rdfs:subClassOf  [ a                            owl:Restriction ;
                           owl:minQualifiedCardinality  "0"^^xsd:nonNegativeInteger ;
                           owl:onClass                  <http://www.uia.no/jpn/tilt#Vital_sign_finding> ;
                           owl:onProperty               <http://www.uia.no/jpn/tilt#hasCurrentVitalSigns>
                         ] .

<http://www.uia.no/jpn/tilt#Pulse_rate_finding>
        a                    owl:Class ;
        rdfs:comment         "Pulse rate finding (finding)\n\nSCTID: 301147003\n\n301147003 | Pulse rate finding (finding) |\n  en   Pulse rate finding\n  en   Pulse rate finding (finding)\n  en   Observation of pulse rate" ;
        rdfs:subClassOf      <http://www.uia.no/jpn/tilt#Pulse_finding> ;
        owl:equivalentClass  [ a               owl:Restriction ;
                               owl:hasValue    "301147003"^^xsd:long ;
                               owl:onProperty  <http://www.uia.no/jpn/tilt#hasSCTID>
                             ] .

<http://www.uia.no/jpn/tilt#Respiratory_measure>
        a                    owl:Class ;
        rdfs:comment         "Respiratory measure (observable entity)\n\nSCTID: 251880004\n\n251880004 | Respiratory measure (observable entity) |\n  en   Respiratory measure\n  en   Respiratory measurements\n  en   Respiratory measure (observable entity)\n  en   Observation of measures of respiratory function" ;
        rdfs:subClassOf      <http://www.uia.no/jpn/tilt#Respiration_observable> ;
        owl:equivalentClass  [ a               owl:Restriction ;
                               owl:hasValue    "251880004"^^xsd:long ;
                               owl:onProperty  <http://www.uia.no/jpn/tilt#hasSCTID>
                             ] .

<http://www.uia.no/jpn/tilt#CharlieData_11_Value>
        a       <http://www.uia.no/jpn/tilt#Value> ;
        <http://www.uia.no/jpn/tilt#hasTime>
                "1063" ;
        <http://www.uia.no/jpn/tilt#hasValueType>
                "xsd:float" ;
        <http://www.uia.no/jpn/tilt#hasValueUnit>
                "Unit" ;
        <http://www.uia.no/jpn/tilt#hasValueValue>
                "551.0" .

<http://www.uia.no/jpn/tilt#CharlieData_2_Value>
        a       <http://www.uia.no/jpn/tilt#Value> ;
        <http://www.uia.no/jpn/tilt#hasTime>
                "5236" ;
        <http://www.uia.no/jpn/tilt#hasValueType>
                "xsd:float" ;
        <http://www.uia.no/jpn/tilt#hasValueUnit>
                "Unit" ;
        <http://www.uia.no/jpn/tilt#hasValueValue>
                "436.0" .

<http://www.uia.no/jpn/tilt#isAbout>
        a       owl:ObjectProperty .

<http://www.uia.no/jpn/tilt#CharlieData_24_Value>
        a       <http://www.uia.no/jpn/tilt#Value> ;
        <http://www.uia.no/jpn/tilt#hasTime>
                "625" ;
        <http://www.uia.no/jpn/tilt#hasValueType>
                "xsd:float" ;
        <http://www.uia.no/jpn/tilt#hasValueUnit>
                "Unit" ;
        <http://www.uia.no/jpn/tilt#hasValueValue>
                "103.0" .

<http://www.uia.no/jpn/tilt#SNOWMEDCTSimulatedinput>
        a                owl:Class ;
        rdfs:subClassOf  <http://www.uia.no/jpn/tilt#CodedSimulatedInputData> .

<http://www.uia.no/jpn/tilt#hasObservableEntity>
        a            owl:ObjectProperty ;
        rdfs:domain  <http://www.uia.no/jpn/tilt#Human> ;
        rdfs:range   <http://www.uia.no/jpn/tilt#Observable_entity> .

<http://www.uia.no/jpn/tilt#Drug_Marevan_ActiveIngredient_Warfarinnatrium>
        a       <http://www.uia.no/jpn/tilt#ActiveIngredient> , owl:NamedIndividual ;
        <http://www.uia.no/jpn/tilt#hasDrug>
                <http://www.uia.no/jpn/tilt#Drug_Marevan_Drug> ;
        <http://www.uia.no/jpn/tilt#hasDrugClass>
                <http://www.uia.no/jpn/tilt#DrugClass_Warfarin> ;
        <http://www.uia.no/jpn/tilt#hasIngredientName>
                "Warfarinnatrium" .

<http://www.uia.no/jpn/tilt#hasDosageForm>
        a                   owl:FunctionalProperty , owl:DatatypeProperty ;
        rdfs:domain         <http://www.uia.no/jpn/tilt#Drug> ;
        rdfs:range          xsd:string ;
        rdfs:subPropertyOf  owl:topDataProperty .

<http://www.uia.no/jpn/tilt#Mental_state,_behavior_and/or_psychosocial_function_finding>
        a                    owl:Class ;
        rdfs:comment         "Mental state, behavior and/or psychosocial function finding (finding)\n\nSCTID: 384821006\n\n384821006 | Mental state, behavior and/or psychosocial function finding (finding) |\n  en   Mental state, behavior and/or psychosocial function finding (finding)\n  en   Mental state, behaviour and/or psychosocial function finding\n  en   Mental state, behavior and/or psychosocial function finding\n  en   Mental state, behaviour and/or psychosocial functioning observations\n  en   Mental state, behavior and/or psychosocial functioning observations" ;
        rdfs:subClassOf      <http://www.uia.no/jpn/tilt#Clinical_history_and_observation_finding> ;
        owl:equivalentClass  [ a               owl:Restriction ;
                               owl:hasValue    "384821006"^^xsd:long ;
                               owl:onProperty  <http://www.uia.no/jpn/tilt#hasSCTID>
                             ] .

<http://www.uia.no/jpn/tilt#CharlieData_20_Value>
        a       <http://www.uia.no/jpn/tilt#Value> ;
        <http://www.uia.no/jpn/tilt#hasTime>
                "76" ;
        <http://www.uia.no/jpn/tilt#hasValueType>
                "xsd:float" ;
        <http://www.uia.no/jpn/tilt#hasValueUnit>
                "Unit" ;
        <http://www.uia.no/jpn/tilt#hasValueValue>
                "1376.0" .

<http://www.uia.no/jpn/tilt#CharlieData_14>
        a       <http://www.uia.no/jpn/tilt#SNOWMEDCTSimulatedinput> ;
        <http://www.uia.no/jpn/tilt#hasSCTID>
                "301147003"^^xsd:long ;
        <http://www.uia.no/jpn/tilt#hasTypeName>
                "Pulse_rate_finding" ;
        <http://www.uia.no/jpn/tilt#hasValue>
                <http://www.uia.no/jpn/tilt#CharlieData_14_Value> .

<http://www.uia.no/jpn/tilt#CharlieData_2>
        a       <http://www.uia.no/jpn/tilt#SNOWMEDCTSimulatedinput> ;
        <http://www.uia.no/jpn/tilt#hasSCTID>
                "5467003"^^xsd:long ;
        <http://www.uia.no/jpn/tilt#hasTypeName>
                "Normal_respiratory_rhythm" ;
        <http://www.uia.no/jpn/tilt#hasValue>
                <http://www.uia.no/jpn/tilt#CharlieData_2_Value> .

<http://www.uia.no/jpn/tilt#Cardiovascular_mesure>
        a                    owl:Class ;
        rdfs:comment         "Cardiovascular measure (observable entity)\n\nSCTID: 310611001\n\n310611001 | Cardiovascular measure (observable entity) |\n  en   Cardiovascular measure\n  en   Cardiovascular measurement\n  en   Cardiovascular measure (observable entity)\n  en   Cardiovascular measurement - observation" ;
        rdfs:subClassOf      <http://www.uia.no/jpn/tilt#Cardiovascular_observable> ;
        owl:equivalentClass  [ a               owl:Restriction ;
                               owl:hasValue    "310611001"^^xsd:long ;
                               owl:onProperty  <http://www.uia.no/jpn/tilt#hasSCTID>
                             ] .

<http://www.uia.no/jpn/tilt#Blood_pressure_finding>
        a                    owl:Class ;
        rdfs:comment         "Blood pressure finding (finding)\n\nSCTID: 392570002\n\n392570002 | Blood pressure finding (finding) |\n  en   Blood pressure finding (finding)\n  en   Blood pressure finding" ;
        rdfs:subClassOf      <http://www.uia.no/jpn/tilt#Vital_sign_finding> ;
        owl:equivalentClass  [ a               owl:Restriction ;
                               owl:hasValue    "392570002"^^xsd:long ;
                               owl:onProperty  <http://www.uia.no/jpn/tilt#hasSCTID>
                             ] .

<http://www.uia.no/jpn/tilt#Drug_Marevan_InactiveIngredient_Lactose>
        a       <http://www.uia.no/jpn/tilt#InactiveIngredient> , owl:NamedIndividual ;
        <http://www.uia.no/jpn/tilt#hasDrug>
                <http://www.uia.no/jpn/tilt#Drug_Marevan_Drug> ;
        <http://www.uia.no/jpn/tilt#hasIngredientName>
                "Lactose" .

<http://www.uia.no/jpn/tilt#Drug_Euthyrox_ActiveIngredient_Levotyroksinnatrium>
        a       <http://www.uia.no/jpn/tilt#ActiveIngredient> , owl:NamedIndividual ;
        <http://www.uia.no/jpn/tilt#hasDrug>
                <http://www.uia.no/jpn/tilt#Drug_Euthyrox_Drug> ;
        <http://www.uia.no/jpn/tilt#hasDrugClass>
                <http://www.uia.no/jpn/tilt#DrugClass_Analgesics> ;
        <http://www.uia.no/jpn/tilt#hasIngredientName>
                "Levotyroksinnatrium" .

<http://www.uia.no/jpn/tilt#Blood_vessel_feature>
        a                    owl:Class ;
        rdfs:comment         "Blood vessel feature (observable entity)\n\nSCTID: 364087003\n\n364087003 | Blood vessel feature (observable entity) |\n  en   Blood vessel feature\n  en   Blood vessel feature (observable entity)" ;
        rdfs:subClassOf      <http://www.uia.no/jpn/tilt#Cardiovascular_observable> ;
        owl:equivalentClass  [ a               owl:Restriction ;
                               owl:hasValue    "364087003"^^xsd:long ;
                               owl:onProperty  <http://www.uia.no/jpn/tilt#hasSCTID>
                             ] .

<http://www.uia.no/jpn/tilt#CharlieData_22>
        a       <http://www.uia.no/jpn/tilt#SNOWMEDCTSimulatedinput> ;
        <http://www.uia.no/jpn/tilt#hasSCTID>
                "163030003"^^xsd:long ;
        <http://www.uia.no/jpn/tilt#hasTypeName>
                "On_examination_Systolic_blood_pressure_reading" ;
        <http://www.uia.no/jpn/tilt#hasValue>
                <http://www.uia.no/jpn/tilt#CharlieData_22_Value> .

<http://www.uia.no/jpn/tilt#ActiveIngredient>
        a                owl:Class ;
        rdfs:subClassOf  <http://www.uia.no/jpn/tilt#Ingredient> .

[ a       owl:Ontology ] .

<http://www.uia.no/jpn/tilt#Body_temperature_finding>
        a                    owl:Class ;
        rdfs:comment         "Body temperature finding (finding)\n\nSCTID: 105723007\n\n105723007 | Body temperature finding (finding) |\n  en   Body temperature finding\n  en   Body temperature finding (finding)" ;
        rdfs:subClassOf      <http://www.uia.no/jpn/tilt#Vital_sign_finding> ;
        owl:equivalentClass  [ a               owl:Restriction ;
                               owl:hasValue    "105723007"^^xsd:long ;
                               owl:onProperty  <http://www.uia.no/jpn/tilt#hasSCTID>
                             ] .

<http://www.uia.no/jpn/tilt#hasActiveIngredient>
        a              owl:ObjectProperty ;
        rdfs:domain    <http://www.uia.no/jpn/tilt#DrugClass> ;
        rdfs:range     <http://www.uia.no/jpn/tilt#ActiveIngredient> ;
        owl:inverseOf  <http://www.uia.no/jpn/tilt#hasDrugClass> .

<http://www.uia.no/jpn/tilt#Drug_Levaxin_Value>
        a       <http://www.uia.no/jpn/tilt#Value> , owl:NamedIndividual ;
        <http://www.uia.no/jpn/tilt#hasValueUnit>
                "μg" ;
        <http://www.uia.no/jpn/tilt#hasValueValue>
                "25" .

<http://www.uia.no/jpn/tilt#CharlieData_18_Value>
        a       <http://www.uia.no/jpn/tilt#Value> ;
        <http://www.uia.no/jpn/tilt#hasTime>
                "5000" ;
        <http://www.uia.no/jpn/tilt#hasValueType>
                "xsd:float" ;
        <http://www.uia.no/jpn/tilt#hasValueUnit>
                "Unit" ;
        <http://www.uia.no/jpn/tilt#hasValueValue>
                "89.95" .

<http://www.uia.no/jpn/tilt#Apnea>
        a                    owl:Class ;
        rdfs:comment         "Apnea (finding)\n\nSCTID: 1023001\n\n1023001 | Apnea (finding) |\n  en   Apnea\n  en   Apnoeic\n  en   Apnoea\n  en   Apneic\n  en   Has stopped breathing\n  en   Not breathing\n  en   Apnea (finding)" ;
        rdfs:subClassOf      <http://www.uia.no/jpn/tilt#Respiratory_rate_AND/OR_rhythm_finding> ;
        owl:equivalentClass  [ a               owl:Restriction ;
                               owl:hasValue    "1023001"^^xsd:long ;
                               owl:onProperty  <http://www.uia.no/jpn/tilt#hasSCTID>
                             ] .

<http://www.uia.no/jpn/tilt#CharlieData_9_Value>
        a       <http://www.uia.no/jpn/tilt#Value> ;
        <http://www.uia.no/jpn/tilt#hasTime>
                "3675" ;
        <http://www.uia.no/jpn/tilt#hasValueType>
                "xsd:float" ;
        <http://www.uia.no/jpn/tilt#hasValueUnit>
                "Unit" ;
        <http://www.uia.no/jpn/tilt#hasValueValue>
                "36.0" .

<http://www.uia.no/jpn/tilt#Drug>
        a                owl:Class ;
        rdfs:subClassOf  [ a                            owl:Restriction ;
                           owl:minQualifiedCardinality  "1"^^xsd:nonNegativeInteger ;
                           owl:onClass                  <http://www.uia.no/jpn/tilt#Ingredient> ;
                           owl:onProperty               <http://www.uia.no/jpn/tilt#hasIngredient>
                         ] ;
        rdfs:subClassOf  [ a                   owl:Class ;
                           owl:intersectionOf  ( [ a                            owl:Restriction ;
                                                   owl:maxQualifiedCardinality  "1"^^xsd:nonNegativeInteger ;
                                                   owl:onClass                  <http://www.uia.no/jpn/tilt#Value> ;
                                                   owl:onProperty               <http://www.uia.no/jpn/tilt#hasDefinedDailyDose>
                                                 ]
                                                 [ a                         owl:Restriction ;
                                                   owl:onDataRange           xsd:string ;
                                                   owl:onProperty            <http://www.uia.no/jpn/tilt#hasArticleNumber> ;
                                                   owl:qualifiedCardinality  "1"^^xsd:nonNegativeInteger
                                                 ]
                                                 [ a                         owl:Restriction ;
                                                   owl:onDataRange           [ a                   rdfs:Datatype ;
                                                                               owl:intersectionOf  ( xsd:string
                                                                                                     [ a          rdfs:Datatype ;
                                                                                                       owl:oneOf  [ a          rdf:List ;
                                                                                                                    rdf:first  "capsule" ;
                                                                                                                    rdf:rest   [ a          rdf:List ;
                                                                                                                                 rdf:first  "other" ;
                                                                                                                                 rdf:rest   [ a          rdf:List ;
                                                                                                                                              rdf:first  "pills" ;
                                                                                                                                              rdf:rest   [ a          rdf:List ;
                                                                                                                                                           rdf:first  "suppository" ;
                                                                                                                                                           rdf:rest   [ a          rdf:List ;
                                                                                                                                                                        rdf:first  "tablets" ;
                                                                                                                                                                        rdf:rest   ()
                                                                                                                                                                      ]
                                                                                                                                                         ]
                                                                                                                                            ]
                                                                                                                               ]
                                                                                                                  ]
                                                                                                     ]
                                                                                                   )
                                                                             ] ;
                                                   owl:onProperty            <http://www.uia.no/jpn/tilt#hasDosageForm> ;
                                                   owl:qualifiedCardinality  "1"^^xsd:nonNegativeInteger
                                                 ]
                                                 [ a                         owl:Restriction ;
                                                   owl:onDataRange           xsd:string ;
                                                   owl:onProperty            <http://www.uia.no/jpn/tilt#hasDrugName> ;
                                                   owl:qualifiedCardinality  "1"^^xsd:nonNegativeInteger
                                                 ]
                                                 [ a                         owl:Restriction ;
                                                   owl:onDataRange           xsd:string ;
                                                   owl:onProperty            <http://www.uia.no/jpn/tilt#hasNumOfDosageForms> ;
                                                   owl:qualifiedCardinality  "1"^^xsd:nonNegativeInteger
                                                 ]
                                               )
                         ] .

owl:Thing  rdfs:comment  "This is the second oblig in the course IKT437 - deadline 9.10.18" .

<http://www.uia.no/jpn/tilt#CharlieData_17>
        a       <http://www.uia.no/jpn/tilt#SNOWMEDCTSimulatedinput> ;
        <http://www.uia.no/jpn/tilt#hasSCTID>
                "310356000"^^xsd:long ;
        <http://www.uia.no/jpn/tilt#hasTypeName>
                "On_examination_Arterial_pressure_index_normal" ;
        <http://www.uia.no/jpn/tilt#hasValue>
                <http://www.uia.no/jpn/tilt#CharlieData_17_Value> .

<http://www.uia.no/jpn/tilt#CharlieData_5>
        a       <http://www.uia.no/jpn/tilt#SNOWMEDCTSimulatedinput> ;
        <http://www.uia.no/jpn/tilt#hasSCTID>
                "163030003"^^xsd:long ;
        <http://www.uia.no/jpn/tilt#hasTypeName>
                "On_examination_Systolic_blood_pressure_reading" ;
        <http://www.uia.no/jpn/tilt#hasValue>
                <http://www.uia.no/jpn/tilt#CharlieData_5_Value> .

<http://www.uia.no/jpn/tilt#CharlieData_14_Value>
        a       <http://www.uia.no/jpn/tilt#Value> ;
        <http://www.uia.no/jpn/tilt#hasTime>
                "343" ;
        <http://www.uia.no/jpn/tilt#hasValueType>
                "xsd:float" ;
        <http://www.uia.no/jpn/tilt#hasValueUnit>
                "Unit" ;
        <http://www.uia.no/jpn/tilt#hasValueValue>
                "2836.0" .

<http://www.uia.no/jpn/tilt#hasName>
        a           owl:DatatypeProperty ;
        rdfs:range  xsd:string .

<http://www.uia.no/jpn/tilt#Ingredient>
        a                owl:Class ;
        rdfs:subClassOf  [ a                         owl:Restriction ;
                           owl:onClass               <http://www.uia.no/jpn/tilt#Drug> ;
                           owl:onProperty            <http://www.uia.no/jpn/tilt#hasDrug> ;
                           owl:qualifiedCardinality  "1"^^xsd:nonNegativeInteger
                         ] ;
        rdfs:subClassOf  [ a                   owl:Class ;
                           owl:intersectionOf  ( [ a                            owl:Restriction ;
                                                   owl:maxQualifiedCardinality  "1"^^xsd:nonNegativeInteger ;
                                                   owl:onClass                  <http://www.uia.no/jpn/tilt#Value> ;
                                                   owl:onProperty               <http://www.uia.no/jpn/tilt#hasAmountInOneDosageForm>
                                                 ]
                                                 [ a                         owl:Restriction ;
                                                   owl:onDataRange           xsd:string ;
                                                   owl:onProperty            <http://www.uia.no/jpn/tilt#hasIngredientName> ;
                                                   owl:qualifiedCardinality  "1"^^xsd:nonNegativeInteger
                                                 ]
                                               )
                         ] .

<http://www.uia.no/jpn/tilt#CharlieData_5_Value>
        a       <http://www.uia.no/jpn/tilt#Value> ;
        <http://www.uia.no/jpn/tilt#hasTime>
                "43" ;
        <http://www.uia.no/jpn/tilt#hasValueType>
                "xsd:float" ;
        <http://www.uia.no/jpn/tilt#hasValueUnit>
                "Unit" ;
        <http://www.uia.no/jpn/tilt#hasValueValue>
                "236.0" .

<http://www.uia.no/jpn/tilt#hasAge>
        a                   owl:DatatypeProperty ;
        rdfs:range          xsd:int ;
        rdfs:subPropertyOf  owl:topDataProperty .

<http://www.uia.no/jpn/tilt#Charlie_Start_Finding_of_rate_of_respiration_finding_Value>
        a       <http://www.uia.no/jpn/tilt#Value> ;
        <http://www.uia.no/jpn/tilt#hasTime>
                "0" ;
        <http://www.uia.no/jpn/tilt#hasValueType>
                "xsd:float" ;
        <http://www.uia.no/jpn/tilt#hasValueUnit>
                "Unit" ;
        <http://www.uia.no/jpn/tilt#hasValueValue>
                "50.0" .

<http://www.uia.no/jpn/tilt#hasDrugClasses>
        a              owl:ObjectProperty ;
        rdfs:domain    <http://www.uia.no/jpn/tilt#Interaction> ;
        rdfs:range     <http://www.uia.no/jpn/tilt#DrugClass> ;
        owl:inverseOf  <http://www.uia.no/jpn/tilt#hasInteraction> .

<http://www.uia.no/jpn/tilt#Charlie_Start_Finding_of_temperature_of_skin>
        a       <http://www.uia.no/jpn/tilt#Finding_of_temperature_of_skin> ;
        <http://www.uia.no/jpn/tilt#hasSCTID>
                "297976006"^^xsd:long ;
        <http://www.uia.no/jpn/tilt#hasValue>
                <http://www.uia.no/jpn/tilt#Charlie_Start_Finding_of_temperature_of_skin_Value> .

<http://www.uia.no/jpn/tilt#General_finding_of_observation_of_patient>
        a                    owl:Class ;
        rdfs:comment         "General finding of observation of patient (finding)\n\nSCTID: 118222006\n\n118222006 | General finding of observation of patient (finding) |\n  en   General finding of observation of patient\n  en   General observation of patient\n  en   General condition of patient\n  en   General finding of observation of patient (finding)" ;
        rdfs:subClassOf      <http://www.uia.no/jpn/tilt#Clinical_history_and_observation_finding> ;
        owl:equivalentClass  [ a               owl:Restriction ;
                               owl:hasValue    "118222006"^^xsd:long ;
                               owl:onProperty  <http://www.uia.no/jpn/tilt#hasSCTID>
                             ] .

<http://www.uia.no/jpn/tilt#DrugClass>
        a                owl:Class ;
        rdfs:subClassOf  [ a                         owl:Restriction ;
                           owl:onDataRange           xsd:string ;
                           owl:onProperty            <http://www.uia.no/jpn/tilt#hasDrugClassName> ;
                           owl:qualifiedCardinality  "1"^^xsd:nonNegativeInteger
                         ] ;
        rdfs:subClassOf  [ a                            owl:Restriction ;
                           owl:minQualifiedCardinality  "0"^^xsd:nonNegativeInteger ;
                           owl:onClass                  <http://www.uia.no/jpn/tilt#Interaction> ;
                           owl:onProperty               <http://www.uia.no/jpn/tilt#hasInteraction>
                         ] ;
        rdfs:subClassOf  [ a                            owl:Restriction ;
                           owl:minQualifiedCardinality  "1"^^xsd:nonNegativeInteger ;
                           owl:onClass                  <http://www.uia.no/jpn/tilt#ActiveIngredient> ;
                           owl:onProperty               <http://www.uia.no/jpn/tilt#hasActiveIngredient>
                         ] .

<http://www.uia.no/jpn/tilt#CharlieData_25>
        a       <http://www.uia.no/jpn/tilt#SNOWMEDCTSimulatedinput> ;
        <http://www.uia.no/jpn/tilt#hasSCTID>
                "170581003"^^xsd:long ;
        <http://www.uia.no/jpn/tilt#hasTypeName>
                "On_examination_initial_high_blood_pressure" ;
        <http://www.uia.no/jpn/tilt#hasValue>
                <http://www.uia.no/jpn/tilt#CharlieData_25_Value> .

<http://www.uia.no/jpn/tilt#CharlieData_10_Value>
        a       <http://www.uia.no/jpn/tilt#Value> ;
        <http://www.uia.no/jpn/tilt#hasTime>
                "3735" ;
        <http://www.uia.no/jpn/tilt#hasValueType>
                "xsd:float" ;
        <http://www.uia.no/jpn/tilt#hasValueUnit>
                "Unit" ;
        <http://www.uia.no/jpn/tilt#hasValueValue>
                "1717.17" .

<http://www.uia.no/jpn/tilt#CharlieData_1_Value>
        a       <http://www.uia.no/jpn/tilt#Value> ;
        <http://www.uia.no/jpn/tilt#hasTime>
                "2345" ;
        <http://www.uia.no/jpn/tilt#hasValueType>
                "xsd:float" ;
        <http://www.uia.no/jpn/tilt#hasValueUnit>
                "Unit" ;
        <http://www.uia.no/jpn/tilt#hasValueValue>
                "765.0" .

<http://www.uia.no/jpn/tilt#Finding_of_response_to_pain>
        a                    owl:Class ;
        rdfs:comment         "Finding of response to pain (finding)\n\nSCTID: 427304006\n\n427304006 | Finding of response to pain (finding) |\n  en   Finding of response to pain (finding)\n  en   Finding of response to pain" ;
        rdfs:subClassOf      <http://www.uia.no/jpn/tilt#Pain> ;
        owl:equivalentClass  [ a               owl:Restriction ;
                               owl:hasValue    "427304006"^^xsd:long ;
                               owl:onProperty  <http://www.uia.no/jpn/tilt#hasSCTID>
                             ] .

<http://www.uia.no/jpn/tilt#hasDrugClass>
        a            owl:ObjectProperty ;
        rdfs:domain  <http://www.uia.no/jpn/tilt#ActiveIngredient> ;
        rdfs:range   <http://www.uia.no/jpn/tilt#DrugClass> .

<http://www.uia.no/jpn/tilt#Charlie_Start_Pulse_rate_finding>
        a       <http://www.uia.no/jpn/tilt#Pulse_rate_finding> ;
        <http://www.uia.no/jpn/tilt#hasSCTID>
                "301147003"^^xsd:long ;
        <http://www.uia.no/jpn/tilt#hasValue>
                <http://www.uia.no/jpn/tilt#Charlie_Start_Pulse_rate_finding_Value> .

<http://www.uia.no/jpn/tilt#CharlieData_23_Value>
        a       <http://www.uia.no/jpn/tilt#Value> ;
        <http://www.uia.no/jpn/tilt#hasTime>
                "26" ;
        <http://www.uia.no/jpn/tilt#hasValueType>
                "xsd:float" ;
        <http://www.uia.no/jpn/tilt#hasValueUnit>
                "Unit" ;
        <http://www.uia.no/jpn/tilt#hasValueValue>
                "110.0" .

<http://www.uia.no/jpn/tilt#Consciousness_and/or_awareness_finding>
        a                    owl:Class ;
        rdfs:comment         "Consciousness and/or awareness finding (finding)\n\nSCTID: 365929007\n\n365929007 | Consciousness and/or awareness finding (finding) |\n  en   Consciousness and/or awareness finding\n  en   Consciousness and/or awareness finding (finding)" ;
        rdfs:subClassOf      <http://www.uia.no/jpn/tilt#Mentalstate_state_finding> ;
        owl:equivalentClass  [ a               owl:Restriction ;
                               owl:hasValue    "365929007"^^xsd:long ;
                               owl:onProperty  <http://www.uia.no/jpn/tilt#hasSCTID>
                             ] .

<http://www.uia.no/jpn/tilt#Awake>
        a                    owl:Class ;
        rdfs:comment         "Awake (finding)\n\nSCTID: 248218005\n\n248218005 | Awake (finding) |\n  en   Awake\n  en   Clear consciousness\n  en   Wide awake\n  en   Awake (finding)" ;
        rdfs:subClassOf      <http://www.uia.no/jpn/tilt#Consciousness_related_finding> ;
        owl:equivalentClass  [ a               owl:Restriction ;
                               owl:hasValue    "248218005"^^xsd:long ;
                               owl:onProperty  <http://www.uia.no/jpn/tilt#hasSCTID>
                             ] .

<http://www.uia.no/jpn/tilt#CharlieData_12>
        a       <http://www.uia.no/jpn/tilt#SNOWMEDCTSimulatedinput> ;
        <http://www.uia.no/jpn/tilt#hasSCTID>
                "297976006"^^xsd:long ;
        <http://www.uia.no/jpn/tilt#hasTypeName>
                "Finding_of_temperature_of_skin" ;
        <http://www.uia.no/jpn/tilt#hasValue>
                <http://www.uia.no/jpn/tilt#CharlieData_12_Value> .

<http://www.uia.no/jpn/tilt#hasSCTID>
        a                   owl:DatatypeProperty ;
        rdfs:domain         <http://www.uia.no/jpn/tilt#SNOMED_CT_CONCEPT> ;
        rdfs:range          xsd:long ;
        rdfs:subPropertyOf  owl:topDataProperty .

<http://www.uia.no/jpn/tilt#hasTime>
        a                   owl:FunctionalProperty , owl:DatatypeProperty ;
        rdfs:domain         <http://www.uia.no/jpn/tilt#Value> ;
        rdfs:range          xsd:long ;
        rdfs:subPropertyOf  owl:topDataProperty .

<http://www.uia.no/jpn/tilt#Cardiovascular_observable>
        a                    owl:Class ;
        rdfs:comment         "Cardiovascular observable (observable entity)\n\nSCTID: 364066008\n\n364066008 | Cardiovascular observable (observable entity) |\n  en   Cardiovascular observable\n  en   Cardiovascular observable (observable entity)" ;
        rdfs:subClassOf      <http://www.uia.no/jpn/tilt#Clinical_history_examination_observable> ;
        owl:equivalentClass  [ a               owl:Restriction ;
                               owl:hasValue    "364066008"^^xsd:long ;
                               owl:onProperty  <http://www.uia.no/jpn/tilt#hasSCTID>
                             ] .

<http://www.uia.no/jpn/tilt#SimulatedInputDataSequence>
        a                owl:Class ;
        rdfs:subClassOf  [ a                         owl:Restriction ;
                           owl:onDataRange           xsd:string ;
                           owl:onProperty            <http://www.uia.no/jpn/tilt#hasName> ;
                           owl:qualifiedCardinality  "1"^^xsd:nonNegativeInteger
                         ] ;
        rdfs:subClassOf  [ a                            owl:Restriction ;
                           owl:minQualifiedCardinality  "0"^^xsd:nonNegativeInteger ;
                           owl:onClass                  <http://www.uia.no/jpn/tilt#SimulatedInputData> ;
                           owl:onProperty               <http://www.uia.no/jpn/tilt#hasSimulatedInputData>
                         ] .

<http://www.uia.no/jpn/tilt#hasNumOfDosageForms>
        a                   owl:FunctionalProperty , owl:DatatypeProperty ;
        rdfs:domain         <http://www.uia.no/jpn/tilt#Drug> ;
        rdfs:range          xsd:string ;
        rdfs:subPropertyOf  owl:topDataProperty .

<http://www.uia.no/jpn/tilt#Neurological_finding>
        a                    owl:Class ;
        rdfs:comment         "Neurological finding (finding)\n\nSCTID: 102957003\n\n102957003 | Neurological finding (finding) |\n  en   Neurological finding\n  en   Neurological findings\n  en   Neurological observations\n  en   Neuro-obs\n  en   Neurological finding (finding)\n  en   Nervous system finding" ;
        rdfs:subClassOf      <http://www.uia.no/jpn/tilt#Clinical_finding> ;
        owl:equivalentClass  [ a               owl:Restriction ;
                               owl:hasValue    "102957003"^^xsd:long ;
                               owl:onProperty  <http://www.uia.no/jpn/tilt#hasSCTID>
                             ] .

<http://www.uia.no/jpn/tilt#CharlieData_20>
        a       <http://www.uia.no/jpn/tilt#SNOWMEDCTSimulatedinput> ;
        <http://www.uia.no/jpn/tilt#hasSCTID>
                "301283003"^^xsd:long ;
        <http://www.uia.no/jpn/tilt#hasTypeName>
                "Finding_of_rate_of_respiration_finding" ;
        <http://www.uia.no/jpn/tilt#hasValue>
                <http://www.uia.no/jpn/tilt#CharlieData_20_Value> .

<http://www.uia.no/jpn/tilt#CharlieData_8>
        a       <http://www.uia.no/jpn/tilt#SNOWMEDCTSimulatedinput> ;
        <http://www.uia.no/jpn/tilt#hasSCTID>
                "301283003"^^xsd:long ;
        <http://www.uia.no/jpn/tilt#hasTypeName>
                "Finding_of_rate_of_respiration_finding" ;
        <http://www.uia.no/jpn/tilt#hasValue>
                <http://www.uia.no/jpn/tilt#CharlieData_8_Value> .

<http://www.uia.no/jpn/tilt#Clinical_history_examination_observable>
        a                    owl:Class ;
        rdfs:comment         "Clinical history/examination observable (observable entity)\n\nSCTID: 363788007\n\n363788007 | Clinical history/examination observable (observable entity) |\n  en   Clinical history/examination observable (observable entity)\n  en   Clinical history/examination observable" ;
        rdfs:subClassOf      <http://www.uia.no/jpn/tilt#Observable_entity> ;
        owl:equivalentClass  [ a               owl:Restriction ;
                               owl:hasValue    "363788007"^^xsd:long ;
                               owl:onProperty  <http://www.uia.no/jpn/tilt#hasSCTID>
                             ] .

<http://www.uia.no/jpn/tilt#Blood_pressure>
        a                    owl:Class ;
        rdfs:comment         "Blood pressure (observable entity)\n\nSCTID: 75367002\n\n75367002 | Blood pressure (observable entity) |\n  en   Blood pressure\n  en   Blood pressure (observable entity)\n  en   BP - Blood pressure" ;
        rdfs:subClassOf      <http://www.uia.no/jpn/tilt#Cardiovascular_mesure> ;
        owl:equivalentClass  [ a               owl:Restriction ;
                               owl:hasValue    "75367002"^^xsd:long ;
                               owl:onProperty  <http://www.uia.no/jpn/tilt#hasSCTID>
                             ] .

<http://www.uia.no/jpn/tilt#Sensory_nervous_system_finding>
        a                    owl:Class ;
        rdfs:comment         "Sensory nervous system finding (finding)\n\nSCTID: 106147001\n\n106147001 | Sensory nervous system finding (finding) |\n  en   Sensory nervous system finding\n  en   Sensory nervous system finding (finding)" ;
        rdfs:subClassOf      <http://www.uia.no/jpn/tilt#Neurological_finding> ;
        owl:equivalentClass  [ a               owl:Restriction ;
                               owl:hasValue    "106147001"^^xsd:long ;
                               owl:onProperty  <http://www.uia.no/jpn/tilt#hasSCTID>
                             ] .

<http://www.uia.no/jpn/tilt#hasDrugName>
        a                   owl:FunctionalProperty , owl:DatatypeProperty ;
        rdfs:domain         <http://www.uia.no/jpn/tilt#Drug> ;
        rdfs:range          xsd:string ;
        rdfs:subPropertyOf  owl:topDataProperty .

<http://www.uia.no/jpn/tilt#hasValueUnit>
        a                   owl:FunctionalProperty , owl:DatatypeProperty ;
        rdfs:domain         <http://www.uia.no/jpn/tilt#Value> ;
        rdfs:range          xsd:string ;
        rdfs:subPropertyOf  owl:topDataProperty .

<http://www.uia.no/jpn/tilt#Vascular_measure>
        a                    owl:Class ;
        rdfs:comment         "Vascular measure (observable entity)\n\nSCTID: 252059006\n\n252059006 | Vascular measure (observable entity) |\n  en   Vascular measure\n  en   Vascular measurements\n  en   Vascular measure (observable entity)" ;
        rdfs:subClassOf      <http://www.uia.no/jpn/tilt#Cardiovascular_mesure> , <http://www.uia.no/jpn/tilt#Blood_vessel_feature> ;
        owl:equivalentClass  [ a               owl:Restriction ;
                               owl:hasValue    "252059006"^^xsd:long ;
                               owl:onProperty  <http://www.uia.no/jpn/tilt#hasSCTID>
                             ] .

<http://www.uia.no/jpn/tilt#SimulatedInputData>
        a                owl:Class ;
        rdfs:subClassOf  [ a                   owl:Class ;
                           owl:intersectionOf  ( [ a                         owl:Restriction ;
                                                   owl:onClass               <http://www.uia.no/jpn/tilt#Value> ;
                                                   owl:onProperty            <http://www.uia.no/jpn/tilt#hasValue> ;
                                                   owl:qualifiedCardinality  "1"^^xsd:nonNegativeInteger
                                                 ]
                                                 [ a                         owl:Restriction ;
                                                   owl:onDataRange           xsd:string ;
                                                   owl:onProperty            <http://www.uia.no/jpn/tilt#hasTypeName> ;
                                                   owl:qualifiedCardinality  "1"^^xsd:nonNegativeInteger
                                                 ]
                                               )
                         ] .

<http://www.uia.no/jpn/tilt#hasValue>
        a           owl:InverseFunctionalProperty , owl:ObjectProperty ;
        rdfs:range  <http://www.uia.no/jpn/tilt#Value> .

<http://www.uia.no/jpn/tilt#On_examination_initial_high_blood_pressure>
        a                    owl:Class ;
        rdfs:comment         "On examination - initial high blood pressure (finding)\n\nSCTID: 170581003\n\n170581003 | On examination - initial high blood pressure (finding) |\n  en   O/E - initial high BP\n  en   On examination - initial high blood pressure (finding)\n  en   On examination - initial high blood pressure\n  en   On examination - initial high BP" ;
        rdfs:subClassOf      <http://www.uia.no/jpn/tilt#Finding_of_systemic_arterial_pressure> ;
        owl:equivalentClass  [ a               owl:Restriction ;
                               owl:hasValue    "170581003"^^xsd:long ;
                               owl:onProperty  <http://www.uia.no/jpn/tilt#hasSCTID>
                             ] .

<http://www.uia.no/jpn/tilt#Charlie_Start_Finding_of_rate_of_respiration_finding>
        a       <http://www.uia.no/jpn/tilt#Finding_of_rate_of_respiration_finding> ;
        <http://www.uia.no/jpn/tilt#hasSCTID>
                "301283003"^^xsd:long ;
        <http://www.uia.no/jpn/tilt#hasValue>
                <http://www.uia.no/jpn/tilt#Charlie_Start_Finding_of_rate_of_respiration_finding_Value> .

<http://www.uia.no/jpn/tilt#Charlie_Start_Pulse_rate_finding_Value>
        a       <http://www.uia.no/jpn/tilt#Value> ;
        <http://www.uia.no/jpn/tilt#hasTime>
                "0" ;
        <http://www.uia.no/jpn/tilt#hasValueType>
                "xsd:float" ;
        <http://www.uia.no/jpn/tilt#hasValueUnit>
                "Unit" ;
        <http://www.uia.no/jpn/tilt#hasValueValue>
                "90.0" .

<http://www.uia.no/jpn/tilt#Unresponsive>
        a                    owl:Class ;
        rdfs:comment         "Unresponsive (finding)\n\nSCTID: 422768004\n\n422768004 | Unresponsive (finding) |\n  en   Unresponsive (finding)\n  en   Unresponsive" ;
        rdfs:subClassOf      <http://www.uia.no/jpn/tilt#Finding_of_mental_alertness> ;
        owl:equivalentClass  [ a               owl:Restriction ;
                               owl:hasValue    "422768004"^^xsd:long ;
                               owl:onProperty  <http://www.uia.no/jpn/tilt#hasSCTID>
                             ] .

<http://www.uia.no/jpn/tilt#CharlieData_17_Value>
        a       <http://www.uia.no/jpn/tilt#Value> ;
        <http://www.uia.no/jpn/tilt#hasTime>
                "1538" ;
        <http://www.uia.no/jpn/tilt#hasValueType>
                "xsd:float" ;
        <http://www.uia.no/jpn/tilt#hasValueUnit>
                "Unit" ;
        <http://www.uia.no/jpn/tilt#hasValueValue>
                "195.72" .

<http://www.uia.no/jpn/tilt#Interaction>
        a                owl:Class ;
        rdfs:subClassOf  [ a                            owl:Restriction ;
                           owl:minQualifiedCardinality  "2"^^xsd:nonNegativeInteger ;
                           owl:onClass                  <http://www.uia.no/jpn/tilt#DrugClass> ;
                           owl:onProperty               <http://www.uia.no/jpn/tilt#hasDrugClasses>
                         ] ;
        rdfs:subClassOf  [ a                   owl:Class ;
                           owl:intersectionOf  ( [ a                         owl:Restriction ;
                                                   owl:onDataRange           xsd:string ;
                                                   owl:onProperty            <http://www.uia.no/jpn/tilt#hasInteractionDescription> ;
                                                   owl:qualifiedCardinality  "1"^^xsd:nonNegativeInteger
                                                 ]
                                                 [ a                         owl:Restriction ;
                                                   owl:onDataRange           xsd:string ;
                                                   owl:onProperty            <http://www.uia.no/jpn/tilt#hasInteractionName> ;
                                                   owl:qualifiedCardinality  "1"^^xsd:nonNegativeInteger
                                                 ]
                                               )
                         ] .

<http://www.uia.no/jpn/tilt#hasValueType>
        a                   owl:FunctionalProperty , owl:DatatypeProperty ;
        rdfs:domain         <http://www.uia.no/jpn/tilt#Value> ;
        rdfs:range          xsd:string ;
        rdfs:subPropertyOf  owl:topDataProperty .

<http://www.uia.no/jpn/tilt#DrugSimulatedInputData>
        a                owl:Class ;
        rdfs:subClassOf  <http://www.uia.no/jpn/tilt#CodedSimulatedInputData> ;
        rdfs:subClassOf  [ a                         owl:Restriction ;
                           owl:onDataRange           xsd:string ;
                           owl:onProperty            <http://www.uia.no/jpn/tilt#hasArticleNumber> ;
                           owl:qualifiedCardinality  "1"^^xsd:nonNegativeInteger
                         ] .

<http://www.uia.no/jpn/tilt#CharlieData_8_Value>
        a       <http://www.uia.no/jpn/tilt#Value> ;
        <http://www.uia.no/jpn/tilt#hasTime>
                "463" ;
        <http://www.uia.no/jpn/tilt#hasValueType>
                "xsd:float" ;
        <http://www.uia.no/jpn/tilt#hasValueUnit>
                "Unit" ;
        <http://www.uia.no/jpn/tilt#hasValueValue>
                "63.0" .

<http://www.uia.no/jpn/tilt#CharlieData_15>
        a       <http://www.uia.no/jpn/tilt#SNOWMEDCTSimulatedinput> ;
        <http://www.uia.no/jpn/tilt#hasSCTID>
                "5467003"^^xsd:long ;
        <http://www.uia.no/jpn/tilt#hasTypeName>
                "Normal_respiratory_rhythm" ;
        <http://www.uia.no/jpn/tilt#hasValue>
                <http://www.uia.no/jpn/tilt#CharlieData_15_Value> .

<http://www.uia.no/jpn/tilt#CharlieData_3>
        a       <http://www.uia.no/jpn/tilt#SNOWMEDCTSimulatedinput> ;
        <http://www.uia.no/jpn/tilt#hasSCTID>
                "297976006"^^xsd:long ;
        <http://www.uia.no/jpn/tilt#hasTypeName>
                "Finding_of_temperature_of_skin" ;
        <http://www.uia.no/jpn/tilt#hasValue>
                <http://www.uia.no/jpn/tilt#CharlieData_3_Value> .

<http://www.uia.no/jpn/tilt#Charlie_Start_Finding_of_temperature_of_skin_Value>
        a       <http://www.uia.no/jpn/tilt#Value> ;
        <http://www.uia.no/jpn/tilt#hasTime>
                "0" ;
        <http://www.uia.no/jpn/tilt#hasValueType>
                "xsd:float" ;
        <http://www.uia.no/jpn/tilt#hasValueUnit>
                "Unit" ;
        <http://www.uia.no/jpn/tilt#hasValueValue>
                "30.0" .

<http://www.uia.no/jpn/tilt#hasIngredientName>
        a                   owl:FunctionalProperty , owl:DatatypeProperty ;
        rdfs:domain         <http://www.uia.no/jpn/tilt#Ingredient> ;
        rdfs:range          xsd:string ;
        rdfs:subPropertyOf  owl:topDataProperty .

<http://www.uia.no/jpn/tilt#CharlieData_13_Value>
        a       <http://www.uia.no/jpn/tilt#Value> ;
        <http://www.uia.no/jpn/tilt#hasTime>
                "742" ;
        <http://www.uia.no/jpn/tilt#hasValueType>
                "xsd:float" ;
        <http://www.uia.no/jpn/tilt#hasValueUnit>
                "Unit" ;
        <http://www.uia.no/jpn/tilt#hasValueValue>
                "923.0" .

<http://www.uia.no/jpn/tilt#hasTypeName>
        a            owl:DatatypeProperty ;
        rdfs:domain  <http://www.uia.no/jpn/tilt#SimulatedInputData> ;
        rdfs:range   xsd:string .

<http://www.uia.no/jpn/tilt#CharlieData_4_Value>
        a       <http://www.uia.no/jpn/tilt#Value> ;
        <http://www.uia.no/jpn/tilt#hasTime>
                "4527" ;
        <http://www.uia.no/jpn/tilt#hasValueType>
                "xsd:float" ;
        <http://www.uia.no/jpn/tilt#hasValueUnit>
                "Unit" ;
        <http://www.uia.no/jpn/tilt#hasValueValue>
                "36.0" .

<http://www.uia.no/jpn/tilt#CharlieData_23>
        a       <http://www.uia.no/jpn/tilt#SNOWMEDCTSimulatedinput> ;
        <http://www.uia.no/jpn/tilt#hasSCTID>
                "301283003"^^xsd:long ;
        <http://www.uia.no/jpn/tilt#hasTypeName>
                "Finding_of_rate_of_respiration_finding" ;
        <http://www.uia.no/jpn/tilt#hasValue>
                <http://www.uia.no/jpn/tilt#CharlieData_23_Value> .

<http://www.uia.no/jpn/tilt#CharlieData_26_Value>
        a       <http://www.uia.no/jpn/tilt#Value> ;
        <http://www.uia.no/jpn/tilt#hasTime>
                "2532" ;
        <http://www.uia.no/jpn/tilt#hasValueType>
                "xsd:float" ;
        <http://www.uia.no/jpn/tilt#hasValueUnit>
                "Unit" ;
        <http://www.uia.no/jpn/tilt#hasValueValue>
                "23.0" .

<http://www.uia.no/jpn/tilt#Finding_of_mental_alertness>
        a                    owl:Class ;
        rdfs:comment         "Finding of mental alertness (finding)\n\nSCTID: 365933000\n\n365933000 | Finding of mental alertness (finding) |\n  en   Mental alertness - finding\n  en   Finding of mental alertness (finding)\n  en   Finding of mental alertness" ;
        rdfs:subClassOf      <http://www.uia.no/jpn/tilt#Consciousness_and/or_awareness_finding> ;
        owl:equivalentClass  [ a               owl:Restriction ;
                               owl:hasValue    "365933000"^^xsd:long ;
                               owl:onProperty  <http://www.uia.no/jpn/tilt#hasSCTID>
                             ] .

<http://www.uia.no/jpn/tilt#hasCurrentVitalSigns>
        a            owl:ObjectProperty ;
        rdfs:domain  <http://www.uia.no/jpn/tilt#HumanState> ;
        rdfs:range   <http://www.uia.no/jpn/tilt#Vital_sign_finding> .

<http://www.uia.no/jpn/tilt#Systolic_blood_pressure>
        a                    owl:Class ;
        rdfs:comment         "Systolic blood pressure (observable entity)\n\nSCTID: 271649006\n\n271649006 | Systolic blood pressure (observable entity) |\n  en   Systolic blood pressure\n  en   Systolic blood pressure (observable entity)\n  en   SAP - Systolic arterial pressure" ;
        rdfs:subClassOf      <http://www.uia.no/jpn/tilt#Vascular_measure> , <http://www.uia.no/jpn/tilt#Blood_pressure> ;
        owl:equivalentClass  [ a               owl:Restriction ;
                               owl:hasValue    "271649006"^^xsd:long ;
                               owl:onProperty  <http://www.uia.no/jpn/tilt#hasSCTID>
                             ] .

<http://www.uia.no/jpn/tilt#hasValueValue>
        a                   owl:FunctionalProperty , owl:DatatypeProperty ;
        rdfs:domain         <http://www.uia.no/jpn/tilt#Value> ;
        rdfs:range          xsd:string ;
        rdfs:subPropertyOf  owl:topDataProperty .

<http://www.uia.no/jpn/tilt#Pulse_finding>
        a                    owl:Class ;
        rdfs:comment         "Pulse finding (finding)\n\nSCTID: 366199006\n\n366199006 | Pulse finding (finding) |\n  en   Pulse finding\n  en   Pulse finding (finding)" ;
        rdfs:subClassOf      <http://www.uia.no/jpn/tilt#Vital_sign_finding> ;
        owl:equivalentClass  [ a               owl:Restriction ;
                               owl:hasValue    "366199006"^^xsd:long ;
                               owl:onProperty  <http://www.uia.no/jpn/tilt#hasSCTID>
                             ] .

<http://www.uia.no/jpn/tilt#CharlieData_22_Value>
        a       <http://www.uia.no/jpn/tilt#Value> ;
        <http://www.uia.no/jpn/tilt#hasTime>
                "9999" ;
        <http://www.uia.no/jpn/tilt#hasValueType>
                "xsd:float" ;
        <http://www.uia.no/jpn/tilt#hasValueUnit>
                "Unit" ;
        <http://www.uia.no/jpn/tilt#hasValueValue>
                "634.0" .

<http://www.uia.no/jpn/tilt#CharlieData_10>
        a       <http://www.uia.no/jpn/tilt#SNOWMEDCTSimulatedinput> ;
        <http://www.uia.no/jpn/tilt#hasSCTID>
                "170581003"^^xsd:long ;
        <http://www.uia.no/jpn/tilt#hasTypeName>
                "On_examination_initial_high_blood_pressure" ;
        <http://www.uia.no/jpn/tilt#hasValue>
                <http://www.uia.no/jpn/tilt#CharlieData_10_Value> .
